update directory structure

theory/JITFlattern.thy
@@ -1,294 +1,39 @@
 theory JITFlattern
 
-imports JITFlattern_aux JITFlattern_prob
+imports JITFlattern_def JITFlattern_aux JITFlattern_prob JITFlattern_aux_l_jump JITFlattern_aux_well_formed JITPer 
 begin
 
-(*
-lemma 
-  assumes a0:"\<forall> x y x' y'. (x,y) \<in> set l_jump \<and> (x',y') \<in> set l_jump \<and> x = x'" and
-  a1:"find_target_pc_in_l_pc l_jump pc = Some npc" and
-  a2:"l_jump \<noteq> []"
-  shows"(pc,npc) \<in> set l_jump"
-proof-
-  have "\<exists> item. item \<in> set l_jump \<and> fst item = pc" using a1 *)
-
-
-lemma search_l_jump:"distinct (map fst l_jump) \<Longrightarrow>
-  find_target_pc_in_l_pc l_jump pc = Some npc \<Longrightarrow>
-  (pc,npc) \<in> set l_jump"
-proof(induct l_jump arbitrary: pc npc)
-  case Nil
-  then show ?case by auto
-next
-  case (Cons a l_jump)
-  assume a0:"find_target_pc_in_l_pc (a # l_jump) pc = Some npc" and
-    c0:"distinct (map fst (a#l_jump))"
-
-  have c1:"distinct (map fst l_jump)" using c0 by auto
-  
-  have c2:"distinct (map fst l_jump) \<Longrightarrow> find_target_pc_in_l_pc l_jump pc = Some npc \<Longrightarrow> (pc, npc) \<in> set l_jump" using Cons by blast
-
-  have a1:"fst a = pc \<or> fst a \<noteq> pc"
-    using word_coorder.extremum word_le_sub1 by blast 
-  thus ?case
-  proof(cases "fst a = pc")
-    case True
-    have "snd a = npc"  by (metis True a0 find_target_pc_in_l_pc.simps(2) fst_conv option.inject snd_conv surj_pair) 
-    then show ?thesis using True by (metis list.set_intros(1) prod.collapse)  
-  next
-    case False
-    have "fst a \<noteq> pc" using False a1 by simp
-    hence "\<exists> x. x \<in> set l_jump \<and> fst x = pc" using a0 c1 c0
-      by (smt (verit, best) Cons.hyps eq_fst_iff find_target_pc_in_l_pc.elims list.distinct(1) list.inject) 
-    then obtain x where b0:"x \<in> set l_jump \<and> fst x = pc" by auto
-    hence "snd x = npc" using a0 c1 c0 c2
-      by (metis False eq_key_imp_eq_value find_target_pc_in_l_pc.simps(2) fstI sndI surj_pair) 
-    then show ?thesis using c1 b0 by (metis list.set_intros(2) prod.collapse) 
-  qed
-qed
-
-(* \<and> fst (lt!idx2)< length l_pc*)
-definition is_increase_list::" ((int\<times>u64) list) \<Rightarrow> (int \<times> nat) list \<Rightarrow> bool" where 
-  "is_increase_list lt lt2 \<equiv> (\<forall> idx1 idx2. idx1<idx2 \<and> idx1\<ge>0 \<and> idx2 < length lt \<longrightarrow> fst (lt!idx1) < fst (lt!idx2)) \<and> 
-    (\<forall> idx. idx \<ge>0 \<and> idx < length lt \<longrightarrow> nat (fst (lt!idx)) <  (length lt2))"
-
-lemma is_increase_list_empty:                              
-  "is_increase_list [] []"
-  apply(unfold is_increase_list_def) by simp
-
-lemma l_jump_elem_increases:
-  "jitflat_bpf lt (l1, l_pc1, l_jump1) = (l, l_pc, l_jump) \<Longrightarrow> 
-  is_increase_list l_jump1 l_pc1  \<Longrightarrow>
-  is_increase_list l_jump l_pc"
-proof(induct lt arbitrary: l1 l_pc1 l_jump1 l l_pc l_jump)
-    case Nil
-    then show ?case by force
-  next
-    case (Cons a lt)
-    assume assm0:"is_increase_list l_jump1 l_pc1" and
-      assm1:"jitflat_bpf (a#lt) (l1, l_pc1, l_jump1) = (l, l_pc, l_jump)" 
-      (*and assm2:"(a#lt) \<noteq> []"*)
-    have "\<exists> l2' l_pc2' l_jump2'. jitflat_bpf [a] (l1,l_pc1,l_jump1) = (l2',l_pc2',l_jump2') \<and>  jitflat_bpf lt (l2',l_pc2',l_jump2') = (l,l_pc,l_jump)"
-      using jitflat_bpf_induct assm1 by blast 
-    then obtain l2' l_pc2' l_jump2' where b0:"jitflat_bpf [a] (l1,l_pc1,l_jump1) = (l2',l_pc2',l_jump2') \<and> jitflat_bpf lt (l2',l_pc2',l_jump2') = (l,l_pc,l_jump)" by auto
-
-    hence "l_jump2' = update_l_jump a l_pc1 l_jump1" using jitflat_bpf.elims by force 
-    hence b1:"l_jump2' = (let (num,off,l_bin0) = a in  if l_bin0!1 = (0x39::u8) then l_jump1@ [(of_nat (length l_pc1), of_nat (length l_pc1) + off)] else l_jump1)" using update_l_jump_def by simp
-    thus ?case
-    proof(cases "(snd (snd a))!1 \<noteq> (0x39::u8)")
-      case True
-      have b2_1:"l_jump2' = l_jump1" using b1 True  by (smt (verit, best) case_prod_conv split_pairs)
-      have b2_2:"length l_pc2' = length l_pc1 + 1" using b0 l_pc_length_prop by force 
-      hence "\<forall> x. x < length l_pc1 \<longrightarrow> x < length l_pc2'" by auto
-      hence "is_increase_list l_jump2' l_pc2'" using assm0 is_increase_list_def b2_1 by simp
-      hence "is_increase_list l_jump l_pc" using b0 Cons.hyps by blast 
-      then show ?thesis by simp
-    next
-      case False
-      have b2_0:"l_jump2' = l_jump1@ [(of_nat (length l_pc1), of_nat (length l_pc1) + (fst (snd a)))]" 
-        using False b1 by (smt (verit, ccfv_threshold) old.prod.case prod.collapse) 
-      hence b3:"\<forall> idx1 idx2. idx1<idx2 \<and> idx1\<ge>0 \<and> idx2 < length l_jump1 \<longrightarrow> fst (l_jump2'!idx1) < fst (l_jump2'!idx2)" using b2_0 assm0
-        by (simp add: is_increase_list_def nth_append)  
-      have b4:"nat (fst (l_jump2'!(length l_jump1))) = (length l_pc1)" using b2_0 by simp
-      have b5:"(\<forall> idx. idx \<ge>0 \<and> idx < length l_jump1 \<longrightarrow> nat (fst (l_jump1!idx)) < (length l_pc1))"
-        using assm0 is_increase_list_def by blast 
-      hence "(\<forall> idx. idx \<ge>0 \<and> idx < length l_jump1 \<longrightarrow> (fst (l_jump1!idx)) < (fst (l_jump2'!(length l_jump1))))"
-        using b4 b5 by (metis zless_nat_conj) 
-      hence b7_1:"(\<forall> idx. idx \<ge>0 \<and> idx < length l_jump1 \<longrightarrow> (fst (l_jump2'!idx)) < (fst (l_jump2'!(length l_jump1))))" by (simp add: b2_0 nth_append) 
-      hence b7:"(\<forall> idx1 idx2. idx1<idx2 \<and> idx1\<ge>0 \<and> idx2 < length l_jump2' \<longrightarrow> fst (l_jump2'!idx1) < fst (l_jump2'!idx2))" 
-        using b7_1 by (metis (no_types, lifting) One_nat_def Suc_eq_plus1 b2_0 b3 length_append less_SucE list.size(3) list.size(4)) 
-
-      have "(\<forall> idx. idx \<ge>0 \<and> idx < length l_jump1 \<longrightarrow> nat (fst (l_jump1!idx)) < (length l_pc2'))"
-        using b5 by (metis b0 l_pc_length_prop trans_less_add2) 
-      hence b6:"(\<forall> idx. idx \<ge>0 \<and> idx < length l_jump2' \<longrightarrow> nat (fst (l_jump2'!idx)) < (length l_pc2'))"
-        by (smt (verit, ccfv_SIG) One_nat_def add.commute b0 b2_0 b4 l_pc_length_prop length_append less_Suc_eq list.size(3) list.size(4) nth_append plus_1_eq_Suc) 
-          
-      hence "is_increase_list l_jump2' l_pc2'"
-        using b6 b7 is_increase_list_def by simp
-      then show ?thesis using b0 Cons by blast
-    qed
-  qed
-
-lemma l_jump_upperbound_aux:
-  "\<exists> lt. jitflat_bpf lt init_second_layer = init_second_layer"
-  apply(unfold init_second_layer_def)
-  using jitflat_bpf.simps(1) by blast 
-
-lemma l_jump_is_distinct:"is_increase_list l_jump1 l_pc1 \<Longrightarrow> \<exists> somelt. jitflat_bpf somelt init_second_layer = (l1, l_pc1, l_jump1) \<Longrightarrow> jitflat_bpf lt (l1, l_pc1, l_jump1) = (l_bin,l_pc,l_jump) \<Longrightarrow> distinct (map fst l_jump1) \<Longrightarrow> distinct (map fst l_jump)"
-proof(induct lt arbitrary: l1 l_pc1 l_jump1 l_bin l_pc l_jump)
-  case Nil
-  then show ?case by simp
-next
-  case (Cons a lt)
-  assume a0:"jitflat_bpf (a#lt) (l1, l_pc1, l_jump1) = (l_bin,l_pc,l_jump)" and 
-  a1:"distinct (map fst l_jump1)" and
-  a2:"\<exists> somelt. jitflat_bpf somelt init_second_layer = (l1, l_pc1, l_jump1)" and
-  a3:"is_increase_list l_jump1 l_pc1"
-  have "\<exists> l2' l_pc2' l_jump2'. jitflat_bpf [a] (l1, l_pc1, l_jump1) = (l2', l_pc2', l_jump2') \<and> 
-         jitflat_bpf lt (l2', l_pc2', l_jump2') = (l_bin,l_pc,l_jump)" using jitflat_bpf_induct a0 by simp
-  then obtain l2' l_pc2' l_jump2' where b0:"jitflat_bpf [a] (l1, l_pc1, l_jump1) = (l2', l_pc2', l_jump2') \<and> 
-         jitflat_bpf lt (l2', l_pc2', l_jump2') = (l_bin,l_pc,l_jump)" by auto
-  hence "l_jump2' = update_l_jump a l_pc1 l_jump1" using jitflat_bpf.elims by force 
-  hence b1:"l_jump2' = (let (num,off,l_bin0) = a in  if l_bin0!1 = (0x39::u8) then l_jump1@ [(of_nat (length l_pc1), of_nat (length l_pc1) + off)] else l_jump1)" using update_l_jump_def by simp
-  obtain somelt where "jitflat_bpf somelt init_second_layer = (l1, l_pc1, l_jump1)" using a2 by auto
-    hence "jitflat_bpf (somelt@[a]) init_second_layer = (l2', l_pc2', l_jump2')"
-       using jitflat_bpf_induct3 b0 by (metis (no_types, opaque_lifting) prod_cases3) 
-    hence b3:"\<exists> somelt. jitflat_bpf somelt init_second_layer = (l2', l_pc2', l_jump2')" by auto
-  thus ?case
-  proof(cases "(snd (snd a))!1 \<noteq> (0x39::u8)")
-    case True
-    have b2_1:"l_jump2' = l_jump1" using b1 True  by (smt (verit, best) case_prod_conv split_pairs)
-    hence b2:"distinct (map fst l_jump2')" using a1 by simp
-    have "is_increase_list l_jump2' l_pc2'" using  l_jump_elem_increases a3 b0 by blast
-    hence "distinct (map fst l_jump)" using b0 b1 b2 Cons a2 b3 b2_1 by simp
-    then show ?thesis using a1 by simp
-  next
-    case False
-    have b2_0:"l_jump2' = l_jump1@ [(of_nat (length l_pc1), of_nat (length l_pc1) + (fst (snd a)))]" 
-      using False b1 by (smt (verit, ccfv_threshold) old.prod.case prod.collapse) 
-    hence " (\<forall> idx. idx \<ge>0 \<and> idx < length l_jump1 \<longrightarrow> nat (fst (l_jump1!idx)) <  (length l_pc1))" using a2 b0 False a3 l_jump_elem_increases a3 b0 is_increase_list_def by blast
-    hence b2_1:" (\<forall> idx. idx \<ge>0 \<and> idx < length l_jump1 \<longrightarrow> nat (fst (l_jump1!idx)) \<noteq>  (length l_pc1))" by fastforce
-    have b2_2:"nat(of_nat (length l_pc1)) = (length l_pc1)" by auto
-    hence "\<forall> elem1 elem2. (elem1,elem2) \<in> set l_jump1 \<longrightarrow> elem1 \<noteq> of_nat (length l_pc1)" using b2_1 b2_2
-      by (metis eq_fst_iff in_set_conv_nth le0) 
-    hence "\<forall> elem1. elem1 \<in> set (map fst l_jump1) \<longrightarrow> elem1 \<noteq> of_nat (length l_pc1)" by auto
-    
-    hence "distinct ((map fst l_jump1) @ [of_nat (length l_pc1)])" using Cons.prems(3)  Cons.prems(4) by auto 
-    hence b2:"distinct (map fst l_jump2')" using b2_0 by simp
-    then show ?thesis using Cons b2 b0 b3 l_jump_elem_increases by blast 
-  qed
-qed
-
-(*
-lemma l_jump_elem_increases:
-  "jitflat_bpf lt init_second_layer = (l_bin,l_pc,l_jump) \<Longrightarrow> 
-  lt \<noteq> [] \<Longrightarrow> 
-  l_jump \<noteq> [] \<Longrightarrow> 
-  \<forall> idx1 idx2. idx1 \<ge>0 \<and> idx1 < length l_jump \<and> idx1 < idx2 \<longrightarrow> fst (l_jump!idx1) < fst (l_jump!idx2)"
-  sorry
-*)
-
-lemma flattern_jump_index_easy:
-  "jitflat_bpf lt (l1,l_pc1,l_jump1) = (l_bin,l_pc,l_jump) \<Longrightarrow>
-  lt!(unat pc) = (num,off,l) \<Longrightarrow>
-  find_target_pc_in_l_pc l_jump (of_nat(length(l_pc1))+uint pc) = Some npc \<Longrightarrow>
-  lt \<noteq> [] \<Longrightarrow>
-  pc = 0 \<Longrightarrow>
-  distinct (map fst l_jump1) \<Longrightarrow>
-  jitflat_bpf somelt init_second_layer = (l1, l_pc1, l_jump1) \<Longrightarrow>
-  is_increase_list l_jump1 l_pc1 \<Longrightarrow>
-  npc = off + (of_nat(length(l_pc1))+pc)"
-proof-
-  assume a0:"jitflat_bpf lt (l1,l_pc1,l_jump1) = (l_bin,l_pc,l_jump)" and
-  a1:"lt!(unat pc) = (num,off,l)" and
-  a2:"find_target_pc_in_l_pc l_jump (int(length(l_pc1))+uint pc) = Some npc" and
-  a3:"lt \<noteq> []" and
-  a4:"pc = 0" and
-  a5:"distinct (map fst l_jump1)" and
-  a6:"jitflat_bpf somelt init_second_layer = (l1, l_pc1, l_jump1)" and
-  a6_1:"is_increase_list l_jump1 l_pc1"
-  let "?xs" = "tl lt"
-  let "?len" = "(length(l_pc1))"
-  have a7:"(num,off,l)#?xs = lt" using a1 a3 a4
-    by (metis list.collapse nth_Cons_0 unat_0) 
-  have b0:"jitflat_bpf ((num,off,l)#?xs) (l1,l_pc1,l_jump1) = (
-  let curr_pc = of_nat (length l1) in 
-  let l_jump' = update_l_jump (num,off,l) l_pc1 l_jump1 in
-      jitflat_bpf ?xs (
-        l1@l,
-        l_pc1@[(curr_pc,num)],
-        l_jump'))" using a0 a4 by auto 
-  have b1_1:"l_jump \<noteq> []" using a2 by force 
-  have b1:"distinct (map fst l_jump)" using l_jump_is_distinct a0 a5 a6 a6_1 by blast
-  have "int ?len = (int(length(l_pc1))+uint pc)" using a4 by simp
-  hence b2:"(int ?len,npc) \<in> set l_jump" using a2 a4 b1 search_l_jump by auto 
-   (* by (metis bot_nat_0.extremum_strict in_set_conv_nth list.size(3) list_in_list.simps(1) list_in_list.simps(2) list_in_list_implies_set_relation) *)
-  have b3:"update_l_jump (num,off,l) l_pc l_jump = (
-  if l!1 = (0x39::u8) then l_jump@ [(of_nat (length l_pc), of_nat (length l_pc) + off)]
-  else l_jump)" 
-    apply(unfold update_l_jump_def Let_def,simp_all) done
-  have b4:"l_jump \<noteq> []" using a2 by auto
-
-  have "l!1 = (0x39::u8) \<or> l!1 \<noteq> (0x39::u8)" by auto
-  thus ?thesis
-  proof(cases "l!1 = (0x39::u8)")
-    case True
-    have c0_0:"update_l_jump (num,off,l) l_pc1 l_jump1 = l_jump1@[(int ?len, of_nat ?len+off)]" using True b0 update_l_jump_def by simp 
-    hence c0_1:"jitflat_bpf ((num,off,l)#?xs) (l1,l_pc1,l_jump1) = (
-        jitflat_bpf ?xs (l1@l,l_pc1@[(of_nat (length l1),num)],l_jump1@[(int ?len, of_nat ?len+off)]))" 
-      using b0 by presburger  
-    have "\<exists> l1' l_pc1' l_jump1'. jitflat_bpf [(num,off,l)] (l1,l_pc1,l_jump1) = (l1',l_pc1',l_jump1') \<and> jitflat_bpf ?xs (l1',l_pc1',l_jump1') = (l_bin,l_pc,l_jump)" 
-      using jitflat_bpf_induct a0 a7 by presburger 
-    then obtain l1' l_pc1' l_jump1' where c0:"jitflat_bpf [(num,off,l)] (l1,l_pc1,l_jump1) = (l1',l_pc1',l_jump1') \<and> jitflat_bpf ?xs (l1',l_pc1',l_jump1') = (l_bin,l_pc,l_jump)" by auto
-    hence c1:"l_jump1' = l_jump1@[(int ?len, of_nat ?len+off)]" using c0 c0_1 c0_0 by simp
-    hence "list_in_list (l_jump1@[(int ?len, of_nat ?len+off)]) 0 l_jump" using a0 a7 not_change_prefix_l_jump b1_1 c1 c0 by blast
-    hence "list_in_list [(int ?len, of_nat ?len+off)] (length l_jump1) l_jump" by (simp add: list_in_list_concat) 
-    hence "(int ?len, of_nat ?len+off) \<in> set l_jump" sorry (*using list_in_list_implies_set_relation by metis*)
-    hence "npc = off + of_nat ?len+pc" using a4 a2 b1 b2 eq_key_imp_eq_value by (metis add.commute add.right_neutral) 
-    then show ?thesis by simp
-  next
-    case False
-    have "update_l_jump (num,off,l) l_pc1 l_jump1 = l_jump1" using False b0 update_l_jump_def by simp
-    hence "jitflat_bpf ((num,off,l)#?xs) (l1,l_pc1,l_jump1) = jitflat_bpf ?xs (l1@l,l_pc1@[(of_nat (length l1),num)],l_jump1)"  using b0 init_second_layer_def by fastforce
-    hence "\<not>(\<exists> x. x \<in> set l_jump \<and> fst x = (int ?len+uint pc))" using b4 a3 a0 l_jump_elem_increases a3 a6 is_increase_list_def a6_1 sorry
-    hence "find_target_pc_in_l_pc l_jump (int ?len+uint pc) = None" using a4 b2 by auto
-
-    then show ?thesis using a2 by fastforce 
-  qed
-qed
-
-lemma flattern_jump_index:
-  "jitflat_bpf lt (l1,l_pc1,l_jump1) = (l_bin,l_pc,l_jump) \<Longrightarrow>
-  lt!(unat pc) = (num,off,l) \<Longrightarrow>
-  distinct (map fst l_jump1) \<Longrightarrow>
-  jitflat_bpf somelt init_second_layer = (l1, l_pc1, l_jump1) \<Longrightarrow>
-  unat pc < length lt \<and> unat pc \<ge> 0  \<Longrightarrow>
-  is_increase_list l_jump1 l_pc1 \<Longrightarrow>
-  find_target_pc_in_l_pc l_jump (of_nat (length l_pc1) + uint pc) = Some npc \<longrightarrow> npc = off + (of_nat (length l_pc1) + pc)"
-  proof(induct lt arbitrary: l1 l_pc1 l_jump1 l_bin l_pc l_jump pc num off l somelt npc)
-    case Nil
-    then show ?case by simp
-  next
-    case (Cons a lt)
-    assume assm0:"jitflat_bpf (a#lt) (l1,l_pc1,l_jump1) = (l_bin,l_pc,l_jump)" and
-      assm1:"(a#lt)!(unat pc) = (num,off,l)" and
-      assm2:"distinct (map fst l_jump1)" and
-      assm3:"unat pc < length (a#lt) \<and> unat pc \<ge> 0" and
-      assm4:"jitflat_bpf somelt init_second_layer = (l1, l_pc1, l_jump1)" and
-      assm5:"is_increase_list l_jump1 l_pc1"
-    have a0:"unat pc = 0 \<or> unat pc \<ge> 1" by auto
-      show ?case
-      proof(cases "unat pc = 0")
-        case True
-        then show ?thesis 
-          using flattern_jump_index_easy True assm0 assm1 assm2 assm3 unat_eq_zero init_second_layer_def
-          using Cons.prems(3) assm0 assm1 flattern_jump_index_easy unat_eq_zero assm4 assm5 by blast
-      next
-        case False
-        have a1:"pc \<ge>1" using False a0 linorder_le_less_linear by force 
-        let "?pc" = "pc -1"
-        have b1:"unat ?pc < length lt \<and> (0::nat) \<le> unat ?pc" using assm3 a1 False unat_sub by fastforce 
-        let "?x" = "tl lt"
-        have b2:"lt ! (unat ?pc) = (num, off, l)" using assm1 False by (simp add: a1 unat_sub)      
-
-        have "\<exists> l2' l_pc2' l_jump2'. jitflat_bpf [a] (l1,l_pc1,l_jump1) = (l2',l_pc2',l_jump2') \<and> jitflat_bpf lt (l2',l_pc2',l_jump2') = (l_bin,l_pc,l_jump)" 
-          using jitflat_bpf_induct assm0 by blast 
-        then obtain l2' l_pc2' l_jump2' where b3_1:"jitflat_bpf [a] (l1,l_pc1,l_jump1) = (l2',l_pc2',l_jump2') \<and> jitflat_bpf lt (l2',l_pc2',l_jump2') = (l_bin,l_pc,l_jump)" by auto
-        
-        have "jitflat_bpf lt (l1,l_pc1,l_jump1) = (l_bin, l_pc, l_jump) \<Longrightarrow> lt ! unat pc = (num, off, l) \<Longrightarrow> distinct (map fst l_jump1) \<Longrightarrow>
-        unat pc < length lt \<and> (0::nat) \<le> unat pc \<Longrightarrow> find_target_pc_in_l_pc l_jump (of_nat (length l_pc1)+ uint pc) = Some npc \<Longrightarrow> npc = off + (of_nat (length l_pc1) + pc)" using Cons by blast
-
-        have b4_0:"jitflat_bpf (somelt@[a]) init_second_layer = (l2',l_pc2',l_jump2')" 
-          using assm4 b3_1 by (metis (no_types, opaque_lifting) jitflat_bpf_induct3 prod_cases3) 
-        have "distinct (map fst l_jump2')" using l_jump_is_distinct b3_1 assm0 assm2 assm4 assm5 by blast
-        hence b4:"find_target_pc_in_l_pc l_jump ((of_nat (length l_pc2'))+uint ?pc) = Some npc \<longrightarrow> npc = off + ((of_nat (length l_pc2'))+?pc)" using Cons b1 b2 b3_1 b4_0 l_jump_elem_increases by blast 
-        have b5:"length l_pc2' = length l_pc1 + 1" using b3_1 l_pc_length_prop by force
-        
-        have "find_target_pc_in_l_pc l_jump ((of_nat (length l_pc1))+uint pc) = Some npc \<longrightarrow> npc = off +  ((of_nat (length l_pc1))+pc)" 
-          using b4 b5 by (smt (verit, best) a1 add.commute diff_add_cancel group_cancel.add2 of_nat_1 of_nat_add uint_sub_lem unsigned_1 word_less_eq_iff_unsigned) 
-        then show ?thesis by force 
-      qed
-    qed
+lemma match_state1_prop:
+  "xst1 = (exec_instr ins sz xpc1 xrs xm xss) \<Longrightarrow> 
+  xst2 = (exec_instr ins sz xpc2 xrs xm xss) \<Longrightarrow>
+  xst1 \<noteq> Stuck \<Longrightarrow>
+  xst2 \<noteq> Stuck \<Longrightarrow>
+  match_state1 xst1 xst2"
+  apply(unfold exec_instr_def match_state1_def,simp_all)
+  apply(cases ins,simp_all)
+        apply(unfold exec_ret_def Let_def)
+        apply(cases "loadv M64 xm (Vptr sp_block (xrs (IR SP) + u64_of_memory_chunk M64))",simp_all)
+  subgoal for a by(cases a,simp_all)
+  subgoal for x7 apply(unfold exec_push_def Let_def)
+    by(cases "storev M64 xm (Vptr sp_block (xrs (IR SP) - u64_of_memory_chunk M64)) (Vlong (xrs (IR x7)))",simp_all)
+  subgoal for x8 apply(unfold exec_pop_def Let_def)
+    apply(cases "loadv M64 xm (Vptr sp_block (xrs (IR SP)))",simp_all)
+    subgoal for a by(cases a,simp_all)
+        done
+      subgoal for x131 x132 apply(cases "eval_testcond x131 xrs",simp_all)
+        done
+      subgoal for x151 x152 x153
+        apply(unfold exec_store_def,simp_all)
+        by(cases "storev x153 xm (Vlong (eval_addrmode64 x151 xrs)) (Vlong (xrs (IR x152)))",simp_all)
+      subgoal for x201 x202 x203 
+        apply(unfold exec_load_def,simp_all)
+        apply(cases "loadv x203 xm (Vlong (eval_addrmode64 x202 xrs))",simp_all)
+        subgoal for a by(cases a,simp_all)
+            done
+          subgoal for x21a 
+            apply(unfold exec_call_def Let_def,simp_all)
+            by(cases "storev M64 xm (Vptr sp_block (xrs (IR SP) - u64_of_memory_chunk M64)) (Vlong (ucast x21a))",simp_all)
+          done
 
 lemma one_step_equiv_layer1:
   assumes a0:"flat_bpf_sem 1 (l_bin,l_pc,l_jump) (pc, fxst) = fxst'" and
@@ -296,15 +41,15 @@ lemma one_step_equiv_layer1:
    a2:"perir_sem 1 lt (pc,xxst) = xxst'" and
    a3:"xxst = Next xpc xrs xm xss" and
    a4:"lt \<noteq> []" and
-   a5:"match_state (pc, xxst) (pc, fxst)" and
+   a5:"JITFlattern_def.match_state (pc, xxst) (pc, fxst)" and
    a6:"snd xxst' \<noteq> Stuck" and
    a7:"unat pc < length lt \<and> unat pc \<ge> 0" and 
    a8:"well_formed_prog lt" and
    a9:"snd fxst' \<noteq> Stuck"
-  shows"match_state xxst' fxst'"
+  shows"JITFlattern_def.match_state xxst' fxst'"
 proof-
   have "\<exists> xpc1. fxst = Next xpc1 xrs xm xss" using a3 a5 
-    apply(unfold match_state_def match_state1_def) 
+    apply(unfold JITFlattern_def.match_state_def match_state1_def) 
     apply(cases fxst,simp_all)
     done
   then obtain xpc1 where a10:"fxst = Next xpc1 xrs xm xss" by auto
@@ -420,6 +165,13 @@ proof-
           (case ss' of None \<Rightarrow> (pc, Stuck) | 
           Some ra \<Rightarrow> (?off, Next xpc rs' xm ra)))" using True b1 b0
         by (smt (z3) False case_prod_conv option.case_eq_if) 
+      have b2_1:"?l \<noteq> []"  using a8 apply(unfold well_formed_prog_def) using b0 a4 a7 by blast
+      hence b2_2:"x64_decode 0 ?l \<noteq> None"  apply(cases "x64_decode 0 ?l",simp_all) sorry
+          (*by (metis (no_types, lifting) Suc_diff_1 option.simps(4) x64_sem.simps(3)) *)
+
+      have "\<exists> d. x64_decode 0 ?l = Some(5, Pcall_i d)" using b2 b2_1 b2_2 is_call_insn b3 by blast 
+      then obtain d where " x64_decode 0 ?l = Some(5, Pcall_i d)" by auto
+      hence "\<forall> n. \<not> (x64_bin_is_sequential n ?l 0)" using x64_bin_is_sequential_x64_decode_pcall_false by blast
       then show ?thesis sorry
     next
       case False
@@ -453,20 +205,48 @@ proof-
             else \<comment>\<open> donot JUMP \<close>
               (pc+1, Next xpc1 rs1 m1 ss1)
           )) " using True a0 c2 a7 c1 a9 by auto    
-                
-          have "\<exists> fxst1. fxst1 = x64_sem ?num l_bin (Next xpc1 xrs xm xss)" by fastforce
-          then obtain fxst1 where d2_0:"fxst1 = x64_sem ?num l_bin (Next xpc1 xrs xm xss)" by auto
-          have "\<exists> xxst1. xxst1 = x64_sem ?num ?l (Next 0 xrs xm xss)" by fastforce
-          then obtain xxst1 where d2_1:"xxst1 = x64_sem ?num ?l (Next 0 xrs xm xss)" by auto
-          have d2:"match_state1 fxst1 xxst1" using d2_0 d2_1 sorry
+        
+        have d4:"(snd (l_pc!(unat pc))) = ?num"
+            by (metis (mono_tags, lifting) a1 a7 b0 flattern_num)         
+        have "\<exists> fxst1. fxst1 = x64_sem ?num l_bin (Next xpc1 xrs xm xss)" by fastforce
+        then obtain fxst1 where d2_0:"fxst1 = x64_sem ?num l_bin (Next xpc1 xrs xm xss)" by auto
+        have "\<exists> xxst1. xxst1 = x64_sem ?num ?l (Next 0 xrs xm xss)" by fastforce
+        then obtain xxst1 where d2_1:"xxst1 = x64_sem ?num ?l (Next 0 xrs xm xss)" by auto
+        have d2_5_1:"xxst1 \<noteq> Stuck" using a6 d1 d2_1 d4 d0 by force
+        hence d2_5:"x64_decode 0 ?l \<noteq> None" using d2_1 apply(cases "x64_decode 0 ?l",simp_all)
+          by (metis (no_types, lifting) Suc_diff_1 bn_2 option.simps(4) x64_sem.simps(3)) 
+
+        have b7_0:"\<exists> src dst. x64_decode 0 ?l = Some(3, Pcmpq_rr src dst)" using is_cmp_insn True bn_1 d2_5 by simp
+        have b7:"?num = 1" using jit_prog_prop2 sorry
+        hence d2_2:"fxst1 = (case x64_decode xpc1 l_bin of
+          None \<Rightarrow> Stuck |
+          Some (sz, ins) \<Rightarrow>
+            x64_sem 0 l_bin (exec_instr ins sz xpc1 xrs xm xss)
+          )" using d2_0 by simp
+        have d2_3_1:"fxst1 \<noteq> Stuck" using a9 d1 d2_0 b0 d4 by auto
+        hence d2_3:"x64_decode xpc1 l_bin \<noteq> None" using d2_2 by(cases "x64_decode xpc1 l_bin",simp_all)
+        hence d2_4:"fxst1 = (case x64_decode xpc1 l_bin of Some (sz, ins) \<Rightarrow> (exec_instr ins sz xpc1 xrs xm xss))" 
+          using d2_2 by force
+
+      
+        have d2_6:"xxst1 = (case x64_decode 0 ?l of Some (sz, ins) \<Rightarrow> (exec_instr ins sz 0 xrs xm xss))"
+          using b7 d2_1 d2_5 by force 
+        
+        have d2_7:"x64_decode 0 ?l = x64_decode xpc1 l_bin" using list_in_list_prop2 d2_3 d2_5 c3_0 by fastforce 
+        have "\<exists> sz ins. x64_decode 0 ?l = Some (sz, ins)" using d2_5 by simp
+        then obtain sz ins where "x64_decode 0 ?l = Some (sz, ins)" by auto
+        hence d2_8:"xxst1 = (exec_instr ins sz 0 xrs xm xss)" using d2_6 by simp
+        hence d2_9:"fxst1 =(exec_instr ins sz xpc1 xrs xm xss)" using d2_0 d2_1 d2_6 d2_4 d2_7
+          by (metis \<open>x64_decode (0::nat) (snd (snd ((lt::(nat \<times> 64 word \<times> 8 word list) list) ! unat (pc::64 word)))) = Some (sz::nat, ins::instruction)\<close> case_prod_conv option.simps(5)) 
+        have d2:"match_state1 fxst1 xxst1" using match_state1_prop d2_3_1 d2_5_1 d2_8 d2_9 by blast
+          
           have d3:"\<exists> xpc' xrs1 xm1 xss1. Next xpc' xrs1 xm1 xss1 = fxst1" 
             using d2 match_state1_def by (smt (verit, ccfv_threshold) outcome.exhaust outcome.simps(5)) 
           then obtain xpc' xrs1 xm1 xss1 where d4_0:"Next xpc' xrs1 xm1 xss1 = fxst1" by auto
           have "\<exists> xpc''. Next xpc'' xrs1 xm1 xss1 = xxst1" 
             using d3 match_state1_def d4_0 by (smt (verit, ccfv_SIG) d2 outcome.exhaust outcome.simps(4) outcome.simps(5))
           then obtain xpc'' where d4_1:"Next xpc'' xrs1 xm1 xss1 = xxst1" by auto
-          have d4:"(snd (l_pc!(unat pc))) = ?num"
-            by (metis (mono_tags, lifting) a1 a7 b0 flattern_num) 
+          
           thus ?thesis
           proof(cases "xrs1 (CR ZF) = 1")
             case True
@@ -476,7 +256,7 @@ proof-
               case True
                 have "\<exists> npc. find_target_pc_in_l_pc l_jump (uint pc) = Some npc" using True by simp
                 then obtain npc where d5_1:"find_target_pc_in_l_pc l_jump (uint pc) = Some npc" by auto
-                hence d5:"npc = ?off+pc" using a1 a4 b0 a7 flattern_jump_index init_second_layer_def l_jump_upperbound_aux is_increase_list_empty
+                hence d5:"npc = ?off+pc" using a1 a4 b0 a7 flattern_jump_index init_second_layer_def is_increase_list_empty
                   by (metis (mono_tags, lifting) add_cancel_left_left distinct.simps(1) list.size(3) map_is_Nil_conv of_nat_unat unsigned_0)                  
                   
                 have d6_0:"fxst' =  (npc, (Next (nat (fst (l_pc!(unat npc)))) xrs1 xm1 xss1))" 
@@ -484,9 +264,9 @@ proof-
                 have d6_1:"xxst' = (?off+pc, xxst1)"
                   by (smt (verit, ccfv_threshold) d0 d2_1 d4_1 d5_0 outcome.simps(4)) 
 
-                have "match_state fxst' xxst'" 
-                  using d6_0 d6_1 match_state_def d4_1 d5 match_state1_def by auto
-                then show ?thesis using match_state_def d6_0 d6_1 match_state1_def \<open>\<And>thesis::bool. (\<And>xpc''::nat. Next xpc'' (xrs1::preg \<Rightarrow> 64 word) (xm1::nat \<Rightarrow> int \<Rightarrow> 8 word option) (xss1::stack_state) = (xxst1::outcome) \<Longrightarrow> thesis) \<Longrightarrow> thesis\<close> by fastforce 
+                have "JITFlattern_def.match_state fxst' xxst'" 
+                  using d6_0 d6_1 JITFlattern_def.match_state_def d4_1 d5 match_state1_def by auto
+                then show ?thesis using JITFlattern_def.match_state_def d6_0 d6_1 match_state1_def \<open>\<And>thesis::bool. (\<And>xpc''::nat. Next xpc'' (xrs1::preg \<Rightarrow> 64 word) (xm1::nat \<Rightarrow> int \<Rightarrow> 8 word option) (xss1::stack_state) = (xxst1::outcome) \<Longrightarrow> thesis) \<Longrightarrow> thesis\<close> by fastforce 
                next
                  case False
                  have "find_target_pc_in_l_pc l_jump (uint pc) = None" using False by simp
@@ -500,7 +280,7 @@ proof-
               have d5_1:"xxst' = (pc+1, xxst1)" by (smt (verit) d0 d2_1 d4_1 d5_0 outcome.simps(4)) 
               have d5_2:"fxst' = (pc+1, fxst1)" 
                 using d5_0 by (smt (verit, ccfv_threshold) d1 d2_0 d4 d4_0 outcome.simps(4)) 
-            then show ?thesis using d5_1 d5_2 match_state_def d2 d3 d4_1 by force 
+            then show ?thesis using d5_1 d5_2 JITFlattern_def.match_state_def d2 d3 d4_1 by force 
         qed
 
         (*hence bn_0:"x64_decode 0 ?l \<noteq> None" using a6 apply(cases "x64_decode 0 ?l",simp_all) using bn_2
@@ -538,14 +318,13 @@ proof-
             by (metis (mono_tags, lifting) flattern_num)
             
 
-          have cn:"match_state1 (snd xxst') (snd fxst')" using c5 d0 c3_0 list_in_list_prop3
-            by (metis add.right_neutral assms(7) snd_conv)
+          have cn:"match_state1 (snd xxst') (snd fxst')" using c5 d0 c3_0 list_in_list_prop3 sorry
+            (*by (metis add.right_neutral assms(7) snd_conv)*)
             
-
           have "fst fxst' = pc+1" using c5 by auto
           moreover have d2:"fst xxst' = pc+1" using d0 by auto
           hence "fst xxst' = fst fxst'" using calculation by presburger 
-          hence "match_state xxst' fxst'" using cn match_state_def match_state1_def 
+          hence "JITFlattern_def.match_state xxst' fxst'" using cn JITFlattern_def.match_state_def match_state1_def 
             apply(cases "snd xxst'",simp_all)
             apply(cases "snd fxst'",simp_all)
             by (simp add: case_prod_beta') 
@@ -595,14 +374,14 @@ lemma n_steps_equiv_layer1:
   perir_sem n lt (pc,xxst) = xxst' \<Longrightarrow>
   xxst = Next xpc xrs xm xss \<Longrightarrow>
   snd xxst' = Next xpc' xrs' xm' xss' \<Longrightarrow>
-  match_state (pc,xxst) (pc,fxst) \<Longrightarrow>
+  JITFlattern_def.match_state (pc,xxst) (pc,fxst) \<Longrightarrow>
   lt \<noteq> [] \<Longrightarrow> 
   well_formed_prog lt \<Longrightarrow>
   snd fxst' = Next xpc'' xrs'' xm'' xss'' \<Longrightarrow>
-  match_state xxst' fxst'"
+  JITFlattern_def.match_state xxst' fxst'"
 proof(induct n arbitrary: prog pc fxst fxst' lt xxst xxst' xpc xrs xm xss xxst' xpc' xrs' xm' xss' xpc'' xrs'' xm'' xss'')
   case 0
-  then show ?case apply(unfold match_state_def,simp_all) 
+  then show ?case apply(unfold JITFlattern_def.match_state_def,simp_all) 
     done
     
 next
@@ -613,7 +392,7 @@ next
   assm3:"xxst = Next xpc xrs xm xss" and
   assm4:"snd xxst' = Next xpc' xrs' xm' xss'" and
   assm5:"lt \<noteq> []" and
-  assm6:"match_state (pc,xxst) (pc,fxst)" and
+  assm6:"JITFlattern_def.match_state (pc,xxst) (pc,fxst)" and
 (*  assm7:"unat pc < length lt \<and> unat pc \<ge> 0" and*)
   assm7:"well_formed_prog lt" and
   assm8:"snd fxst' = Next xpc'' xrs'' xm'' xss''"
@@ -642,11 +421,11 @@ next
 
   hence c0:"(unat pc < length lt \<and> unat pc \<ge> 0)" using l_pc_length_prop  init_second_layer_def assm1
     by (metis add.right_neutral list.size(3) prod.collapse) 
-  have bn:"match_state next_s next_f"
+  have bn:"JITFlattern_def.match_state next_s next_f"
     using one_step_equiv_layer1 b1 assm1 b0 assm3 assm5 assm6 a1 c0 assm8 c0_1 assm7
     by (metis outcome.distinct(1) prod.collapse snd_conv) 
 
-  have a2:"(pc', snd next_f) = next_f" using bn match_state_def a1 b0 b1
+  have a2:"(pc', snd next_f) = next_f" using bn JITFlattern_def.match_state_def a1 b0 b1
     apply(cases "Next xrs1 xpc1 m1 xss1",simp_all)
     apply(cases "snd next_f",simp_all)
     subgoal for x11 x11a x12 x13 x14 by force
@@ -655,11 +434,9 @@ next
 
   have c1:"flat_bpf_sem n prog next_f = fxst'" using flat_bpf_sem_induct_aux2 assm0 b1 by blast
 
-  hence "match_state xxst' fxst'" 
+  hence "JITFlattern_def.match_state xxst' fxst'" 
     using a0 a1 a2 Suc bn c1 assm5 assm4 by metis
   then show ?case by simp
 qed
-
-  
 
 end
