theory/JITFlattern_aux_l_jump.thy
@@ -1,0 +1,256 @@
+theory JITFlattern_aux_l_jump
+  imports JITFlattern_def Proof1 JITFlattern_aux
+begin
+
+lemma search_l_jump:"distinct (map fst l_jump) \<Longrightarrow>
+  find_target_pc_in_l_pc l_jump pc = Some npc \<Longrightarrow>
+  (pc,npc) \<in> set l_jump"
+proof(induct l_jump arbitrary: pc npc)
+  case Nil
+  then show ?case by auto
+next
+  case (Cons a l_jump)
+  assume a0:"find_target_pc_in_l_pc (a # l_jump) pc = Some npc" and
+    c0:"distinct (map fst (a#l_jump))"
+
+  have c1:"distinct (map fst l_jump)" using c0 by auto
+  
+  have c2:"distinct (map fst l_jump) \<Longrightarrow> find_target_pc_in_l_pc l_jump pc = Some npc \<Longrightarrow> (pc, npc) \<in> set l_jump" using Cons by blast
+
+  have a1:"fst a = pc \<or> fst a \<noteq> pc"
+    using word_coorder.extremum word_le_sub1 by blast 
+  thus ?case
+  proof(cases "fst a = pc")
+    case True
+    have "snd a = npc"  by (metis True a0 find_target_pc_in_l_pc.simps(2) fst_conv option.inject snd_conv surj_pair) 
+    then show ?thesis using True by (metis list.set_intros(1) prod.collapse)  
+  next
+    case False
+    have "fst a \<noteq> pc" using False a1 by simp
+    hence "\<exists> x. x \<in> set l_jump \<and> fst x = pc" using a0 c1 c0
+      by (smt (verit, best) Cons.hyps eq_fst_iff find_target_pc_in_l_pc.elims list.distinct(1) list.inject) 
+    then obtain x where b0:"x \<in> set l_jump \<and> fst x = pc" by auto
+    hence "snd x = npc" using a0 c1 c0 c2
+      by (metis False eq_key_imp_eq_value find_target_pc_in_l_pc.simps(2) fstI sndI surj_pair) 
+    then show ?thesis using c1 b0 by (metis list.set_intros(2) prod.collapse) 
+  qed
+qed
+
+(* \<and> fst (lt!idx2)< length l_pc*)
+definition is_increase_list::" ((int\<times>u64) list) \<Rightarrow> (int \<times> nat) list \<Rightarrow> bool" where 
+  "is_increase_list lt lt2 \<equiv> (\<forall> idx1 idx2. idx1<idx2 \<and> idx1\<ge>0 \<and> idx2 < length lt \<longrightarrow> fst (lt!idx1) < fst (lt!idx2)) \<and> 
+    (\<forall> idx. idx \<ge>0 \<and> idx < length lt \<longrightarrow> nat (fst (lt!idx)) <  (length lt2))"
+
+lemma is_increase_list_empty:                              
+  "is_increase_list [] []"
+  apply(unfold is_increase_list_def) by simp
+
+lemma l_jump_elem_increases:
+  "jitflat_bpf lt (l1, l_pc1, l_jump1) = (l, l_pc, l_jump) \<Longrightarrow> 
+  is_increase_list l_jump1 l_pc1  \<Longrightarrow>
+  is_increase_list l_jump l_pc"
+proof(induct lt arbitrary: l1 l_pc1 l_jump1 l l_pc l_jump)
+    case Nil
+    then show ?case by force
+  next
+    case (Cons a lt)
+    assume assm0:"is_increase_list l_jump1 l_pc1" and
+      assm1:"jitflat_bpf (a#lt) (l1, l_pc1, l_jump1) = (l, l_pc, l_jump)" 
+      (*and assm2:"(a#lt) \<noteq> []"*)
+    have "\<exists> l2' l_pc2' l_jump2'. jitflat_bpf [a] (l1,l_pc1,l_jump1) = (l2',l_pc2',l_jump2') \<and>  jitflat_bpf lt (l2',l_pc2',l_jump2') = (l,l_pc,l_jump)"
+      using jitflat_bpf_induct assm1 by blast 
+    then obtain l2' l_pc2' l_jump2' where b0:"jitflat_bpf [a] (l1,l_pc1,l_jump1) = (l2',l_pc2',l_jump2') \<and> jitflat_bpf lt (l2',l_pc2',l_jump2') = (l,l_pc,l_jump)" by auto
+
+    hence "l_jump2' = update_l_jump a l_pc1 l_jump1" using jitflat_bpf.elims by force 
+    hence b1:"l_jump2' = (let (num,off,l_bin0) = a in  if l_bin0!1 = (0x39::u8) then l_jump1@ [(of_nat (length l_pc1), of_nat (length l_pc1) + off)] else l_jump1)" using update_l_jump_def by simp
+    thus ?case
+    proof(cases "(snd (snd a))!1 \<noteq> (0x39::u8)")
+      case True
+      have b2_1:"l_jump2' = l_jump1" using b1 True  by (smt (verit, best) case_prod_conv split_pairs)
+      have b2_2:"length l_pc2' = length l_pc1 + 1" using b0 l_pc_length_prop by force 
+      hence "\<forall> x. x < length l_pc1 \<longrightarrow> x < length l_pc2'" by auto
+      hence "is_increase_list l_jump2' l_pc2'" using assm0 is_increase_list_def b2_1 by simp
+      hence "is_increase_list l_jump l_pc" using b0 Cons.hyps by blast 
+      then show ?thesis by simp
+    next
+      case False
+      have b2_0:"l_jump2' = l_jump1@ [(of_nat (length l_pc1), of_nat (length l_pc1) + (fst (snd a)))]" 
+        using False b1 by (smt (verit, ccfv_threshold) old.prod.case prod.collapse) 
+      hence b3:"\<forall> idx1 idx2. idx1<idx2 \<and> idx1\<ge>0 \<and> idx2 < length l_jump1 \<longrightarrow> fst (l_jump2'!idx1) < fst (l_jump2'!idx2)" using b2_0 assm0
+        by (simp add: is_increase_list_def nth_append)  
+      have b4:"nat (fst (l_jump2'!(length l_jump1))) = (length l_pc1)" using b2_0 by simp
+      have b5:"(\<forall> idx. idx \<ge>0 \<and> idx < length l_jump1 \<longrightarrow> nat (fst (l_jump1!idx)) < (length l_pc1))"
+        using assm0 is_increase_list_def by blast 
+      hence "(\<forall> idx. idx \<ge>0 \<and> idx < length l_jump1 \<longrightarrow> (fst (l_jump1!idx)) < (fst (l_jump2'!(length l_jump1))))"
+        using b4 b5 by (metis zless_nat_conj) 
+      hence b7_1:"(\<forall> idx. idx \<ge>0 \<and> idx < length l_jump1 \<longrightarrow> (fst (l_jump2'!idx)) < (fst (l_jump2'!(length l_jump1))))" by (simp add: b2_0 nth_append) 
+      hence b7:"(\<forall> idx1 idx2. idx1<idx2 \<and> idx1\<ge>0 \<and> idx2 < length l_jump2' \<longrightarrow> fst (l_jump2'!idx1) < fst (l_jump2'!idx2))" 
+        using b7_1 by (metis (no_types, lifting) One_nat_def Suc_eq_plus1 b2_0 b3 length_append less_SucE list.size(3) list.size(4)) 
+
+      have "(\<forall> idx. idx \<ge>0 \<and> idx < length l_jump1 \<longrightarrow> nat (fst (l_jump1!idx)) < (length l_pc2'))"
+        using b5 by (metis b0 l_pc_length_prop trans_less_add2) 
+      hence b6:"(\<forall> idx. idx \<ge>0 \<and> idx < length l_jump2' \<longrightarrow> nat (fst (l_jump2'!idx)) < (length l_pc2'))"
+        by (smt (verit, ccfv_SIG) One_nat_def add.commute b0 b2_0 b4 l_pc_length_prop length_append less_Suc_eq list.size(3) list.size(4) nth_append plus_1_eq_Suc) 
+          
+      hence "is_increase_list l_jump2' l_pc2'"
+        using b6 b7 is_increase_list_def by simp
+      then show ?thesis using b0 Cons by blast
+    qed
+  qed
+
+lemma l_jump_is_distinct:"is_increase_list l_jump1 l_pc1 \<Longrightarrow> jitflat_bpf lt (l1, l_pc1, l_jump1) = (l_bin,l_pc,l_jump) \<Longrightarrow> distinct (map fst l_jump1) \<Longrightarrow> distinct (map fst l_jump)"
+proof(induct lt arbitrary: l1 l_pc1 l_jump1 l_bin l_pc l_jump)
+  case Nil
+  then show ?case by simp
+next
+  case (Cons a lt)
+  assume a0:"jitflat_bpf (a#lt) (l1, l_pc1, l_jump1) = (l_bin,l_pc,l_jump)" and 
+  a1:"distinct (map fst l_jump1)" and
+  a3:"is_increase_list l_jump1 l_pc1"
+  have "\<exists> l2' l_pc2' l_jump2'. jitflat_bpf [a] (l1, l_pc1, l_jump1) = (l2', l_pc2', l_jump2') \<and> 
+         jitflat_bpf lt (l2', l_pc2', l_jump2') = (l_bin,l_pc,l_jump)" using jitflat_bpf_induct a0 by simp
+  then obtain l2' l_pc2' l_jump2' where b0:"jitflat_bpf [a] (l1, l_pc1, l_jump1) = (l2', l_pc2', l_jump2') \<and> 
+         jitflat_bpf lt (l2', l_pc2', l_jump2') = (l_bin,l_pc,l_jump)" by auto
+  hence "l_jump2' = update_l_jump a l_pc1 l_jump1" using jitflat_bpf.elims by force 
+  hence b1:"l_jump2' = (let (num,off,l_bin0) = a in  if l_bin0!1 = (0x39::u8) then l_jump1@ [(of_nat (length l_pc1), of_nat (length l_pc1) + off)] else l_jump1)" using update_l_jump_def by simp
+  thus ?case
+  proof(cases "(snd (snd a))!1 \<noteq> (0x39::u8)")
+    case True
+    have b2_1:"l_jump2' = l_jump1" using b1 True  by (smt (verit, best) case_prod_conv split_pairs)
+    hence b2:"distinct (map fst l_jump2')" using a1 by simp
+    have "is_increase_list l_jump2' l_pc2'" using  l_jump_elem_increases a3 b0 by blast
+    hence "distinct (map fst l_jump)" using b0 b1 b2 Cons b2_1 by blast
+    then show ?thesis using a1 by simp
+  next
+    case False
+    have b2_0:"l_jump2' = l_jump1@ [(of_nat (length l_pc1), of_nat (length l_pc1) + (fst (snd a)))]" 
+      using False b1 by (smt (verit, ccfv_threshold) old.prod.case prod.collapse) 
+    hence " (\<forall> idx. idx \<ge>0 \<and> idx < length l_jump1 \<longrightarrow> nat (fst (l_jump1!idx)) <  (length l_pc1))" using b0 False a3 l_jump_elem_increases a3 b0 is_increase_list_def by blast
+    hence b2_1:" (\<forall> idx. idx \<ge>0 \<and> idx < length l_jump1 \<longrightarrow> nat (fst (l_jump1!idx)) \<noteq>  (length l_pc1))" by fastforce
+    have b2_2:"nat(of_nat (length l_pc1)) = (length l_pc1)" by auto
+    hence "\<forall> elem1 elem2. (elem1,elem2) \<in> set l_jump1 \<longrightarrow> elem1 \<noteq> of_nat (length l_pc1)" using b2_1 b2_2
+      by (metis eq_fst_iff in_set_conv_nth le0) 
+    hence "\<forall> elem1. elem1 \<in> set (map fst l_jump1) \<longrightarrow> elem1 \<noteq> of_nat (length l_pc1)" by auto
+    
+    hence "distinct ((map fst l_jump1) @ [of_nat (length l_pc1)])" using Cons.prems(3) by auto 
+    hence b2:"distinct (map fst l_jump2')" using b2_0 by simp
+    then show ?thesis using Cons b2 b0 l_jump_elem_increases by blast 
+  qed
+qed
+
+
+lemma flattern_jump_index_easy:
+  "jitflat_bpf lt (l1,l_pc1,l_jump1) = (l_bin,l_pc,l_jump) \<Longrightarrow>
+  lt!(unat pc) = (num,off,l) \<Longrightarrow>
+  find_target_pc_in_l_pc l_jump (of_nat(length(l_pc1))+uint pc) = Some npc \<Longrightarrow>
+  lt \<noteq> [] \<Longrightarrow>
+  pc = 0 \<Longrightarrow>
+  distinct (map fst l_jump1) \<Longrightarrow>
+  is_increase_list l_jump1 l_pc1 \<Longrightarrow>
+  npc = off + (of_nat(length(l_pc1))+pc)"
+proof-
+  assume a0:"jitflat_bpf lt (l1,l_pc1,l_jump1) = (l_bin,l_pc,l_jump)" and
+  a1:"lt!(unat pc) = (num,off,l)" and
+  a2:"find_target_pc_in_l_pc l_jump (int(length(l_pc1))+uint pc) = Some npc" and
+  a3:"lt \<noteq> []" and
+  a4:"pc = 0" and
+  a5:"distinct (map fst l_jump1)" and
+  a6:"is_increase_list l_jump1 l_pc1"
+  let "?xs" = "tl lt"
+  let "?len" = "(length(l_pc1))"
+  have a7:"(num,off,l)#?xs = lt" using a1 a3 a4
+    by (metis list.collapse nth_Cons_0 unat_0) 
+  have b0:"jitflat_bpf ((num,off,l)#?xs) (l1,l_pc1,l_jump1) = (
+  let curr_pc = of_nat (length l1) in 
+  let l_jump' = update_l_jump (num,off,l) l_pc1 l_jump1 in
+      jitflat_bpf ?xs (
+        l1@l,
+        l_pc1@[(curr_pc,num)],
+        l_jump'))" using a0 a4 by auto 
+  have b1_1:"l_jump \<noteq> []" using a2 by force 
+  have b1:"distinct (map fst l_jump)" using l_jump_is_distinct a0 a5 a6 by blast
+  have "int ?len = (int(length(l_pc1))+uint pc)" using a4 by simp
+  hence b2:"(int ?len,npc) \<in> set l_jump" using a2 a4 b1 search_l_jump by auto 
+   (* by (metis bot_nat_0.extremum_strict in_set_conv_nth list.size(3) list_in_list.simps(1) list_in_list.simps(2) list_in_list_implies_set_relation) *)
+  have b3:"update_l_jump (num,off,l) l_pc l_jump = (
+  if l!1 = (0x39::u8) then l_jump@ [(of_nat (length l_pc), of_nat (length l_pc) + off)]
+  else l_jump)" 
+    apply(unfold update_l_jump_def Let_def,simp_all) done
+  have b4:"l_jump \<noteq> []" using a2 by auto
+
+  have "l!1 = (0x39::u8) \<or> l!1 \<noteq> (0x39::u8)" by auto
+  thus ?thesis
+  proof(cases "l!1 = (0x39::u8)")
+    case True
+    have c0_0:"update_l_jump (num,off,l) l_pc1 l_jump1 = l_jump1@[(int ?len, of_nat ?len+off)]" using True b0 update_l_jump_def by simp 
+    hence c0_1:"jitflat_bpf ((num,off,l)#?xs) (l1,l_pc1,l_jump1) = (
+        jitflat_bpf ?xs (l1@l,l_pc1@[(of_nat (length l1),num)],l_jump1@[(int ?len, of_nat ?len+off)]))" 
+      using b0 by presburger  
+    have "\<exists> l1' l_pc1' l_jump1'. jitflat_bpf [(num,off,l)] (l1,l_pc1,l_jump1) = (l1',l_pc1',l_jump1') \<and> jitflat_bpf ?xs (l1',l_pc1',l_jump1') = (l_bin,l_pc,l_jump)" 
+      using jitflat_bpf_induct a0 a7 by presburger 
+    then obtain l1' l_pc1' l_jump1' where c0:"jitflat_bpf [(num,off,l)] (l1,l_pc1,l_jump1) = (l1',l_pc1',l_jump1') \<and> jitflat_bpf ?xs (l1',l_pc1',l_jump1') = (l_bin,l_pc,l_jump)" by auto
+    hence c1:"l_jump1' = l_jump1@[(int ?len, of_nat ?len+off)]" using c0 c0_1 c0_0 by simp
+    hence "list_in_list (l_jump1@[(int ?len, of_nat ?len+off)]) 0 l_jump" using a0 a7 not_change_prefix_l_jump b1_1 c1 c0 by blast
+    hence "list_in_list [(int ?len, of_nat ?len+off)] (length l_jump1) l_jump" by (simp add: list_in_list_concat) 
+    hence "(int ?len, of_nat ?len+off) \<in> set l_jump" sorry (*using list_in_list_implies_set_relation by metis*)
+    hence "npc = off + of_nat ?len+pc" using a4 a2 b1 b2 eq_key_imp_eq_value by (metis add.commute add.right_neutral) 
+    then show ?thesis by simp
+  next
+    case False
+    have "update_l_jump (num,off,l) l_pc1 l_jump1 = l_jump1" using False b0 update_l_jump_def by simp
+    hence "jitflat_bpf ((num,off,l)#?xs) (l1,l_pc1,l_jump1) = jitflat_bpf ?xs (l1@l,l_pc1@[(of_nat (length l1),num)],l_jump1)"  using b0 init_second_layer_def by fastforce
+    hence "\<not>(\<exists> x. x \<in> set l_jump \<and> fst x = (int ?len+uint pc))" using b4 a3 a0 l_jump_elem_increases a3 a6 is_increase_list_def a6 sorry
+    hence "find_target_pc_in_l_pc l_jump (int ?len+uint pc) = None" using a4 b2 by auto
+    then show ?thesis using a2 by fastforce 
+  qed
+qed
+
+lemma flattern_jump_index:
+  "jitflat_bpf lt (l1,l_pc1,l_jump1) = (l_bin,l_pc,l_jump) \<Longrightarrow>
+  lt!(unat pc) = (num,off,l) \<Longrightarrow>
+  distinct (map fst l_jump1) \<Longrightarrow>
+  unat pc < length lt \<and> unat pc \<ge> 0  \<Longrightarrow>
+  is_increase_list l_jump1 l_pc1 \<Longrightarrow>
+  find_target_pc_in_l_pc l_jump (of_nat (length l_pc1) + uint pc) = Some npc \<longrightarrow> npc = off + (of_nat (length l_pc1) + pc)"
+  proof(induct lt arbitrary: l1 l_pc1 l_jump1 l_bin l_pc l_jump pc num off l npc)
+    case Nil
+    then show ?case by simp
+  next
+    case (Cons a lt)
+    assume assm0:"jitflat_bpf (a#lt) (l1,l_pc1,l_jump1) = (l_bin,l_pc,l_jump)" and
+      assm1:"(a#lt)!(unat pc) = (num,off,l)" and
+      assm2:"distinct (map fst l_jump1)" and
+      assm3:"unat pc < length (a#lt) \<and> unat pc \<ge> 0" and
+      assm5:"is_increase_list l_jump1 l_pc1"
+    have a0:"unat pc = 0 \<or> unat pc \<ge> 1" by auto
+      show ?case
+      proof(cases "unat pc = 0")
+        case True
+        then show ?thesis 
+          using flattern_jump_index_easy True assm0 assm1 assm2 assm3 unat_eq_zero init_second_layer_def
+          using Cons.prems(3) assm0 assm1 flattern_jump_index_easy unat_eq_zero assm5 by blast
+      next
+        case False
+        have a1:"pc \<ge>1" using False a0 linorder_le_less_linear by force 
+        let "?pc" = "pc -1"
+        have b1:"unat ?pc < length lt \<and> (0::nat) \<le> unat ?pc" using assm3 a1 False unat_sub by fastforce 
+        let "?x" = "tl lt"
+        have b2:"lt ! (unat ?pc) = (num, off, l)" using assm1 False by (simp add: a1 unat_sub)      
+
+        have "\<exists> l2' l_pc2' l_jump2'. jitflat_bpf [a] (l1,l_pc1,l_jump1) = (l2',l_pc2',l_jump2') \<and> jitflat_bpf lt (l2',l_pc2',l_jump2') = (l_bin,l_pc,l_jump)" 
+          using jitflat_bpf_induct assm0 by blast 
+        then obtain l2' l_pc2' l_jump2' where b3_1:"jitflat_bpf [a] (l1,l_pc1,l_jump1) = (l2',l_pc2',l_jump2') \<and> jitflat_bpf lt (l2',l_pc2',l_jump2') = (l_bin,l_pc,l_jump)" by auto
+        
+        have "jitflat_bpf lt (l1,l_pc1,l_jump1) = (l_bin, l_pc, l_jump) \<Longrightarrow> lt ! unat pc = (num, off, l) \<Longrightarrow> distinct (map fst l_jump1) \<Longrightarrow>
+        unat pc < length lt \<and> (0::nat) \<le> unat pc \<Longrightarrow> find_target_pc_in_l_pc l_jump (of_nat (length l_pc1)+ uint pc) = Some npc \<Longrightarrow> npc = off + (of_nat (length l_pc1) + pc)" using Cons by blast
+        have "distinct (map fst l_jump2')" using l_jump_is_distinct b3_1 assm0 assm2  assm5 by blast
+        hence b4:"find_target_pc_in_l_pc l_jump ((of_nat (length l_pc2'))+uint ?pc) = Some npc \<longrightarrow> npc = off + ((of_nat (length l_pc2'))+?pc)" using Cons b1 b2 b3_1 l_jump_elem_increases by blast 
+        have b5:"length l_pc2' = length l_pc1 + 1" using b3_1 l_pc_length_prop by force
+        
+        have "find_target_pc_in_l_pc l_jump ((of_nat (length l_pc1))+uint pc) = Some npc \<longrightarrow> npc = off +  ((of_nat (length l_pc1))+pc)" 
+          using b4 b5 by (smt (verit, best) a1 add.commute diff_add_cancel group_cancel.add2 of_nat_1 of_nat_add uint_sub_lem unsigned_1 word_less_eq_iff_unsigned) 
+        then show ?thesis by force 
+      qed
+    qed
+
+end
