theory/JITFlattern_aux_well_formed.thy
@@ -1,0 +1,665 @@
+theory JITFlattern_aux_well_formed
+  imports JITPer_aux JITFlattern_def
+begin
+
+lemma jit_prog_prop1:"per_jit_ins ins \<noteq> None \<Longrightarrow>
+  \<exists> num off l_bin0. per_jit_ins ins = Some (num,off,l_bin0) \<and> num > 0 "
+  apply(unfold per_jit_ins_def )
+  apply(unfold per_jit_load_reg64_def per_jit_add_reg64_1_def per_jit_add_imm64_1_def  per_jit_sub_reg64_1_def per_jit_mov_reg64_1_def 
+per_jit_or_reg64_1_def per_jit_and_reg64_1_def per_jit_xor_reg64_1_def per_jit_mul_reg64_def per_jit_jcc_def per_jit_shift_lsh_reg64_def per_jit_shift_rsh_reg64_def
+per_jit_shift_arsh_reg64_def per_jit_load_reg64_def  per_jit_store_reg64_def per_jit_call_reg_def per_jit_exit_def Let_def)
+ apply(cases ins,simp_all)
+  subgoal for x31 x32 x33 x34
+    by(cases x33,simp_all)
+  subgoal for x91 x92 x93 
+    apply(cases x91,simp_all)
+             apply(cases x93,simp_all)
+            apply(cases x93,simp_all)
+    apply(cases x93,simp_all)
+    subgoal for x2 by(cases "bpf_to_x64_reg x92",simp_all)
+          apply(cases x93,simp_all)
+         apply(cases x93,simp_all)
+        apply(cases x93,simp_all)
+    subgoal for x2 apply(cases "bpf_to_x64_reg x92",simp_all)
+      by(cases "bpf_to_x64_reg x2",simp_all)
+       apply(cases x93,simp_all)
+    subgoal for x2 apply(cases "bpf_to_x64_reg x92",simp_all) 
+      by(cases "bpf_to_x64_reg x2",simp_all)
+      apply(cases x93,simp_all)
+     apply(cases x93,simp_all)
+    apply(cases x93,simp_all)
+    subgoal for x2 apply(cases "bpf_to_x64_reg x92",simp_all)  
+      by(cases "bpf_to_x64_reg x2",simp_all)
+    done
+  subgoal for x161 x162 x163 x164
+    apply(cases x163,simp_all)
+    subgoal for x2 apply(cases x161,simp_all)
+      by (metis option.discI) 
+    done
+  done
+
+(*lemma jit_prog_prop2:"per_jit_ins ins = Some (num,off,l_bin0) \<Longrightarrow> \<exists> src dst. x64_decode 0 l_bin0 = Some(3, Pcmpq_rr src dst) \<Longrightarrow> l_bin0\<noteq>[] \<Longrightarrow> num = 1"*)
+lemma jit_prog_prop3:
+  "jitper insns = Some lt \<Longrightarrow> 
+  lt \<noteq> [] \<Longrightarrow>
+  lt!(unat pc) = (num,off,l_bin0) \<Longrightarrow> 
+  unat pc < length lt \<and> unat pc \<ge> 0 \<Longrightarrow> 
+  num > 0"
+  sorry
+
+lemma jit_prog_prop2:"per_jit_ins ins = Some (num,off,l_bin0) \<Longrightarrow> \<exists> src dst. x64_decode 0 l_bin0 = Some(3, Pcmpq_rr src dst) \<Longrightarrow>  num = 1"
+  using x64_encode_decode_consistency 
+  apply(unfold per_jit_ins_def,simp_all)
+apply(unfold per_jit_load_reg64_def per_jit_add_reg64_1_def per_jit_add_imm64_1_def  per_jit_sub_reg64_1_def per_jit_mov_reg64_1_def 
+per_jit_or_reg64_1_def per_jit_and_reg64_1_def per_jit_xor_reg64_1_def per_jit_mul_reg64_def per_jit_jcc_def per_jit_shift_lsh_reg64_def per_jit_shift_rsh_reg64_def
+per_jit_shift_arsh_reg64_def per_jit_load_reg64_def  per_jit_store_reg64_def per_jit_call_reg_def per_jit_exit_def Let_def)
+  apply(cases ins,simp_all)
+     prefer 4
+  subgoal for x161 x162 x163 x164
+    apply(cases x163,simp_all)
+    subgoal for x2
+      apply(cases x161,simp_all)
+      apply(split if_splits,simp_all)
+      done
+    done
+
+  subgoal for x21 x22 x23 x24
+    apply(subgoal_tac "x64_decode 0 l_bin0 = Some (12,Pmovl_ri REG_SCRATCH (scast x24))")
+     apply auto[1]
+    apply(subgoal_tac "list_in_list (x64_encode (Pmovl_ri REG_SCRATCH (scast x24))) 0 l_bin0",simp_all)
+    by (metis append.left_neutral list.size(3) list_in_list_prop_aux2)
+
+  subgoal for x31 x32 x33 x34
+    apply(cases x33,simp_all)
+    subgoal for x2
+      apply(subgoal_tac "x64_decode 0 l_bin0 = Some (12,Pmovl_ri REG_SCRATCH (scast x34))")
+       apply auto[1]
+apply(subgoal_tac "list_in_list (x64_encode (Pmovl_ri REG_SCRATCH (scast x34))) 0 l_bin0",simp_all)
+      by (metis append.left_neutral list.size(3) list_in_list_prop_aux2)
+    done
+
+  subgoal for x91 x92 x93
+    apply(cases x91,simp_all)
+             apply(cases x93,simp_all)
+    subgoal for x1
+apply(subgoal_tac "x64_decode 0 l_bin0 = Some (12,Pmovl_ri REG_OTHER_SCRATCH (scast x1))")
+      apply auto[1]
+apply(subgoal_tac "list_in_list (x64_encode (Pmovl_ri REG_OTHER_SCRATCH (scast x1))) 0 l_bin0",simp_all)
+      by (metis append.left_neutral list.size(3) list_in_list_prop_aux2)
+
+            apply(cases x93,simp_all)
+           defer 
+           apply(cases x93,simp_all)
+          apply(cases x93,simp_all)
+         prefer 3 apply(cases x93,simp_all)
+        prefer 3 apply(cases x93,simp_all)
+           apply(cases x93,simp_all)
+    subgoal for x2
+      apply(cases "bpf_to_x64_reg x92",simp_all)
+                     apply(subgoal_tac "x64_decode 0 l_bin0 = Some (1,Ppushl_r RCX)")
+                      apply auto[1]
+                     apply(subgoal_tac "list_in_list (x64_encode (Ppushl_r RCX)) 0 l_bin0",simp_all)
+                     apply (meson list_in_list_concat list_in_list_prop)
+                     apply(subgoal_tac "x64_decode 0 l_bin0 = Some (1,Ppushl_r RCX)")
+                      apply auto[1]
+                     apply(subgoal_tac "list_in_list (x64_encode (Ppushl_r RCX)) 0 l_bin0",simp_all)
+                    apply (meson list_in_list_concat list_in_list_prop)
+                   apply(cases "bpf_to_x64_reg x2",simp_all)
+                          apply(subgoal_tac "x64_decode 0 l_bin0 = Some (1,Ppushl_r RAX)")
+                      apply auto[1]
+                     apply(subgoal_tac "list_in_list (x64_encode (Ppushl_r RAX)) 0 l_bin0",simp_all)
+                          apply (meson list_in_list_concat list_in_list_prop)
+            apply(subgoal_tac "x64_decode 0 l_bin0 = Some (1,Ppushl_r RBX)")
+                      apply auto[1]
+                     apply(subgoal_tac "list_in_list (x64_encode (Ppushl_r RBX)) 0 l_bin0",simp_all)
+                     apply (meson list_in_list_concat list_in_list_prop)
+            apply(subgoal_tac "x64_decode 0 l_bin0 = Some (1,Ppushl_r RDX)")
+                      apply auto[1]
+                     apply(subgoal_tac "list_in_list (x64_encode (Ppushl_r RDX)) 0 l_bin0",simp_all)
+                          apply (meson list_in_list_concat list_in_list_prop)
+            apply(subgoal_tac "x64_decode 0 l_bin0 = Some (1,Ppushl_r RSI)")
+                      apply auto[1]
+                     apply(subgoal_tac "list_in_list (x64_encode (Ppushl_r RSI)) 0 l_bin0",simp_all)
+                     apply (meson list_in_list_concat list_in_list_prop)
+
+            apply(subgoal_tac "x64_decode 0 l_bin0 = Some (1,Ppushl_r RDI)")
+                      apply auto[1]
+                     apply(subgoal_tac "list_in_list (x64_encode (Ppushl_r RDI)) 0 l_bin0",simp_all)
+                          apply (meson list_in_list_concat list_in_list_prop)
+                          apply(subgoal_tac "x64_decode 0 l_bin0 = Some (1,Ppushl_r RBP)")
+                      apply auto[1]
+                     apply(subgoal_tac "list_in_list (x64_encode (Ppushl_r RBP)) 0 l_bin0",simp_all)
+                          apply (meson list_in_list_concat list_in_list_prop)
+              apply(subgoal_tac "x64_decode 0 l_bin0 = Some (1,Ppushl_r SP)")
+                      apply auto[1]
+                     apply(subgoal_tac "list_in_list (x64_encode (Ppushl_r SP)) 0 l_bin0",simp_all)
+                          apply (meson list_in_list_concat list_in_list_prop)
+              apply(subgoal_tac "x64_decode 0 l_bin0 = Some (1,Ppushl_r R8)")
+                      apply auto[1]
+                     apply(subgoal_tac "list_in_list (x64_encode (Ppushl_r R8)) 0 l_bin0",simp_all)
+                          apply (meson list_in_list_concat list_in_list_prop)
+              apply(subgoal_tac "x64_decode 0 l_bin0 = Some (1,Ppushl_r R9)")
+                      apply auto[1]
+                     apply(subgoal_tac "list_in_list (x64_encode (Ppushl_r R9)) 0 l_bin0",simp_all)
+                         apply (meson list_in_list_concat list_in_list_prop)
+              apply(subgoal_tac "x64_decode 0 l_bin0 = Some (1,Ppushl_r REG_OTHER_SCRATCH)")
+                      apply auto[1]
+                     apply(subgoal_tac "list_in_list (x64_encode (Ppushl_r REG_OTHER_SCRATCH)) 0 l_bin0",simp_all)
+                        apply (meson list_in_list_concat list_in_list_prop)
+        apply(subgoal_tac "x64_decode 0 l_bin0 = Some (1,Ppushl_r REG_SCRATCH)")
+                      apply auto[1]
+                     apply(subgoal_tac "list_in_list (x64_encode (Ppushl_r REG_SCRATCH)) 0 l_bin0",simp_all)
+                       apply (meson list_in_list_concat list_in_list_prop)
+        apply(subgoal_tac "x64_decode 0 l_bin0 = Some (1,Ppushl_r R12)")
+                      apply auto[1]
+                     apply(subgoal_tac "list_in_list (x64_encode (Ppushl_r R12)) 0 l_bin0",simp_all)
+                      apply (meson list_in_list_concat list_in_list_prop)
+
+   apply(subgoal_tac "x64_decode 0 l_bin0 = Some (1,Ppushl_r R13)")
+                      apply auto[1]
+                     apply(subgoal_tac "list_in_list (x64_encode (Ppushl_r R13)) 0 l_bin0",simp_all)
+        apply (meson list_in_list_concat list_in_list_prop)
+           apply(subgoal_tac "x64_decode 0 l_bin0 = Some (1,Ppushl_r R14)")
+                      apply auto[1]
+                     apply(subgoal_tac "list_in_list (x64_encode (Ppushl_r R14)) 0 l_bin0",simp_all)
+                    apply (meson list_in_list_concat list_in_list_prop)
+           apply(subgoal_tac "x64_decode 0 l_bin0 = Some (1,Ppushl_r R15)")
+                      apply auto[1]
+                     apply(subgoal_tac "list_in_list (x64_encode (Ppushl_r R15)) 0 l_bin0",simp_all)
+                   apply (meson list_in_list_concat list_in_list_prop)
+           apply(subgoal_tac "x64_decode 0 l_bin0 = Some (1,Ppushl_r RCX)")
+                      apply auto[1]
+                     apply(subgoal_tac "list_in_list (x64_encode (Ppushl_r RCX)) 0 l_bin0",simp_all)
+                  apply (meson list_in_list_concat list_in_list_prop)
+           apply(subgoal_tac "x64_decode 0 l_bin0 = Some (1,Ppushl_r RCX)")
+                      apply auto[1]
+                     apply(subgoal_tac "list_in_list (x64_encode (Ppushl_r RCX)) 0 l_bin0",simp_all)
+        apply (meson list_in_list_concat list_in_list_prop)
+           apply(subgoal_tac "x64_decode 0 l_bin0 = Some (1,Ppushl_r RCX)")
+                      apply auto[1]
+                     apply(subgoal_tac "list_in_list (x64_encode (Ppushl_r RCX)) 0 l_bin0",simp_all)
+        apply (meson list_in_list_concat list_in_list_prop)
+
+           apply(subgoal_tac "x64_decode 0 l_bin0 = Some (1,Ppushl_r RCX)")
+                      apply auto[1]
+                     apply(subgoal_tac "list_in_list (x64_encode (Ppushl_r RCX)) 0 l_bin0",simp_all)
+        apply (meson list_in_list_concat list_in_list_prop)
+
+           apply(subgoal_tac "x64_decode 0 l_bin0 = Some (1,Ppushl_r RCX)")
+                      apply auto[1]
+                     apply(subgoal_tac "list_in_list (x64_encode (Ppushl_r RCX)) 0 l_bin0",simp_all)
+        apply (meson list_in_list_concat list_in_list_prop)
+
+           apply(subgoal_tac "x64_decode 0 l_bin0 = Some (1,Ppushl_r RCX)")
+                      apply auto[1]
+                     apply(subgoal_tac "list_in_list (x64_encode (Ppushl_r RCX)) 0 l_bin0",simp_all)
+        apply (meson list_in_list_concat list_in_list_prop)
+
+           apply(subgoal_tac "x64_decode 0 l_bin0 = Some (1,Ppushl_r RCX)")
+                      apply auto[1]
+                     apply(subgoal_tac "list_in_list (x64_encode (Ppushl_r RCX)) 0 l_bin0",simp_all)
+        apply (meson list_in_list_concat list_in_list_prop)
+
+           apply(subgoal_tac "x64_decode 0 l_bin0 = Some (1,Ppushl_r RCX)")
+                      apply auto[1]
+                     apply(subgoal_tac "list_in_list (x64_encode (Ppushl_r RCX)) 0 l_bin0",simp_all)
+        apply (meson list_in_list_concat list_in_list_prop)
+
+           apply(subgoal_tac "x64_decode 0 l_bin0 = Some (1,Ppushl_r RCX)")
+                      apply auto[1]
+                     apply(subgoal_tac "list_in_list (x64_encode (Ppushl_r RCX)) 0 l_bin0",simp_all)
+        apply (meson list_in_list_concat list_in_list_prop)
+
+           apply(subgoal_tac "x64_decode 0 l_bin0 = Some (1,Ppushl_r RCX)")
+                      apply auto[1]
+                     apply(subgoal_tac "list_in_list (x64_encode (Ppushl_r RCX)) 0 l_bin0",simp_all)
+        apply (meson list_in_list_concat list_in_list_prop)
+
+           apply(subgoal_tac "x64_decode 0 l_bin0 = Some (1,Ppushl_r RCX)")
+                      apply auto[1]
+                     apply(subgoal_tac "list_in_list (x64_encode (Ppushl_r RCX)) 0 l_bin0",simp_all)
+        apply (meson list_in_list_concat list_in_list_prop)
+
+           apply(subgoal_tac "x64_decode 0 l_bin0 = Some (1,Ppushl_r RCX)")
+                      apply auto[1]
+                     apply(subgoal_tac "list_in_list (x64_encode (Ppushl_r RCX)) 0 l_bin0",simp_all)
+        apply (meson list_in_list_concat list_in_list_prop)
+
+           apply(subgoal_tac "x64_decode 0 l_bin0 = Some (1,Ppushl_r RCX)")
+                      apply auto[1]
+                     apply(subgoal_tac "list_in_list (x64_encode (Ppushl_r RCX)) 0 l_bin0",simp_all)
+        apply (meson list_in_list_concat list_in_list_prop)
+      done
+      apply(cases x93,simp_all)
+    subgoal for x2
+      apply(cases "bpf_to_x64_reg x92",simp_all)
+apply(subgoal_tac "x64_decode 0 l_bin0 = Some (1,Ppushl_r RCX)")
+                      apply auto[1]
+                     apply(subgoal_tac "list_in_list (x64_encode (Ppushl_r RCX)) 0 l_bin0",simp_all)
+                     apply (meson list_in_list_concat list_in_list_prop)
+apply(subgoal_tac "x64_decode 0 l_bin0 = Some (1,Ppushl_r RCX)")
+                      apply auto[1]
+                     apply(subgoal_tac "list_in_list (x64_encode (Ppushl_r RCX)) 0 l_bin0",simp_all)
+      apply (meson list_in_list_concat list_in_list_prop)
+                   apply(cases "bpf_to_x64_reg x2",simp_all)
+  apply(subgoal_tac "x64_decode 0 l_bin0 = Some (1,Ppushl_r RAX)")
+                      apply auto[1]
+                     apply(subgoal_tac "list_in_list (x64_encode (Ppushl_r RAX)) 0 l_bin0",simp_all)
+                          apply (meson list_in_list_concat list_in_list_prop)
+            apply(subgoal_tac "x64_decode 0 l_bin0 = Some (1,Ppushl_r RBX)")
+                      apply auto[1]
+                     apply(subgoal_tac "list_in_list (x64_encode (Ppushl_r RBX)) 0 l_bin0",simp_all)
+                     apply (meson list_in_list_concat list_in_list_prop)
+            apply(subgoal_tac "x64_decode 0 l_bin0 = Some (1,Ppushl_r RDX)")
+                      apply auto[1]
+                     apply(subgoal_tac "list_in_list (x64_encode (Ppushl_r RDX)) 0 l_bin0",simp_all)
+                          apply (meson list_in_list_concat list_in_list_prop)
+            apply(subgoal_tac "x64_decode 0 l_bin0 = Some (1,Ppushl_r RSI)")
+                      apply auto[1]
+                     apply(subgoal_tac "list_in_list (x64_encode (Ppushl_r RSI)) 0 l_bin0",simp_all)
+                     apply (meson list_in_list_concat list_in_list_prop)
+
+            apply(subgoal_tac "x64_decode 0 l_bin0 = Some (1,Ppushl_r RDI)")
+                      apply auto[1]
+                     apply(subgoal_tac "list_in_list (x64_encode (Ppushl_r RDI)) 0 l_bin0",simp_all)
+                          apply (meson list_in_list_concat list_in_list_prop)
+                          apply(subgoal_tac "x64_decode 0 l_bin0 = Some (1,Ppushl_r RBP)")
+                      apply auto[1]
+                     apply(subgoal_tac "list_in_list (x64_encode (Ppushl_r RBP)) 0 l_bin0",simp_all)
+                          apply (meson list_in_list_concat list_in_list_prop)
+              apply(subgoal_tac "x64_decode 0 l_bin0 = Some (1,Ppushl_r SP)")
+                      apply auto[1]
+                     apply(subgoal_tac "list_in_list (x64_encode (Ppushl_r SP)) 0 l_bin0",simp_all)
+                          apply (meson list_in_list_concat list_in_list_prop)
+              apply(subgoal_tac "x64_decode 0 l_bin0 = Some (1,Ppushl_r R8)")
+                      apply auto[1]
+                     apply(subgoal_tac "list_in_list (x64_encode (Ppushl_r R8)) 0 l_bin0",simp_all)
+                          apply (meson list_in_list_concat list_in_list_prop)
+              apply(subgoal_tac "x64_decode 0 l_bin0 = Some (1,Ppushl_r R9)")
+                      apply auto[1]
+                     apply(subgoal_tac "list_in_list (x64_encode (Ppushl_r R9)) 0 l_bin0",simp_all)
+                         apply (meson list_in_list_concat list_in_list_prop)
+              apply(subgoal_tac "x64_decode 0 l_bin0 = Some (1,Ppushl_r REG_OTHER_SCRATCH)")
+                      apply auto[1]
+                     apply(subgoal_tac "list_in_list (x64_encode (Ppushl_r REG_OTHER_SCRATCH)) 0 l_bin0",simp_all)
+                        apply (meson list_in_list_concat list_in_list_prop)
+        apply(subgoal_tac "x64_decode 0 l_bin0 = Some (1,Ppushl_r REG_SCRATCH)")
+                      apply auto[1]
+                     apply(subgoal_tac "list_in_list (x64_encode (Ppushl_r REG_SCRATCH)) 0 l_bin0",simp_all)
+                       apply (meson list_in_list_concat list_in_list_prop)
+        apply(subgoal_tac "x64_decode 0 l_bin0 = Some (1,Ppushl_r R12)")
+                      apply auto[1]
+                     apply(subgoal_tac "list_in_list (x64_encode (Ppushl_r R12)) 0 l_bin0",simp_all)
+                      apply (meson list_in_list_concat list_in_list_prop)
+
+   apply(subgoal_tac "x64_decode 0 l_bin0 = Some (1,Ppushl_r R13)")
+                      apply auto[1]
+                     apply(subgoal_tac "list_in_list (x64_encode (Ppushl_r R13)) 0 l_bin0",simp_all)
+        apply (meson list_in_list_concat list_in_list_prop)
+           apply(subgoal_tac "x64_decode 0 l_bin0 = Some (1,Ppushl_r R14)")
+                      apply auto[1]
+                     apply(subgoal_tac "list_in_list (x64_encode (Ppushl_r R14)) 0 l_bin0",simp_all)
+                    apply (meson list_in_list_concat list_in_list_prop)
+           apply(subgoal_tac "x64_decode 0 l_bin0 = Some (1,Ppushl_r R15)")
+                      apply auto[1]
+                     apply(subgoal_tac "list_in_list (x64_encode (Ppushl_r R15)) 0 l_bin0",simp_all)
+                   apply (meson list_in_list_concat list_in_list_prop)
+           apply(subgoal_tac "x64_decode 0 l_bin0 = Some (1,Ppushl_r RCX)")
+                      apply auto[1]
+                     apply(subgoal_tac "list_in_list (x64_encode (Ppushl_r RCX)) 0 l_bin0",simp_all)
+                  apply (meson list_in_list_concat list_in_list_prop)
+           apply(subgoal_tac "x64_decode 0 l_bin0 = Some (1,Ppushl_r RCX)")
+                      apply auto[1]
+                     apply(subgoal_tac "list_in_list (x64_encode (Ppushl_r RCX)) 0 l_bin0",simp_all)
+        apply (meson list_in_list_concat list_in_list_prop)
+           apply(subgoal_tac "x64_decode 0 l_bin0 = Some (1,Ppushl_r RCX)")
+                      apply auto[1]
+                     apply(subgoal_tac "list_in_list (x64_encode (Ppushl_r RCX)) 0 l_bin0",simp_all)
+        apply (meson list_in_list_concat list_in_list_prop)
+
+           apply(subgoal_tac "x64_decode 0 l_bin0 = Some (1,Ppushl_r RCX)")
+                      apply auto[1]
+                     apply(subgoal_tac "list_in_list (x64_encode (Ppushl_r RCX)) 0 l_bin0",simp_all)
+        apply (meson list_in_list_concat list_in_list_prop)
+
+           apply(subgoal_tac "x64_decode 0 l_bin0 = Some (1,Ppushl_r RCX)")
+                      apply auto[1]
+                     apply(subgoal_tac "list_in_list (x64_encode (Ppushl_r RCX)) 0 l_bin0",simp_all)
+        apply (meson list_in_list_concat list_in_list_prop)
+
+           apply(subgoal_tac "x64_decode 0 l_bin0 = Some (1,Ppushl_r RCX)")
+                      apply auto[1]
+                     apply(subgoal_tac "list_in_list (x64_encode (Ppushl_r RCX)) 0 l_bin0",simp_all)
+        apply (meson list_in_list_concat list_in_list_prop)
+
+           apply(subgoal_tac "x64_decode 0 l_bin0 = Some (1,Ppushl_r RCX)")
+                      apply auto[1]
+                     apply(subgoal_tac "list_in_list (x64_encode (Ppushl_r RCX)) 0 l_bin0",simp_all)
+        apply (meson list_in_list_concat list_in_list_prop)
+
+           apply(subgoal_tac "x64_decode 0 l_bin0 = Some (1,Ppushl_r RCX)")
+                      apply auto[1]
+                     apply(subgoal_tac "list_in_list (x64_encode (Ppushl_r RCX)) 0 l_bin0",simp_all)
+        apply (meson list_in_list_concat list_in_list_prop)
+
+           apply(subgoal_tac "x64_decode 0 l_bin0 = Some (1,Ppushl_r RCX)")
+                      apply auto[1]
+                     apply(subgoal_tac "list_in_list (x64_encode (Ppushl_r RCX)) 0 l_bin0",simp_all)
+        apply (meson list_in_list_concat list_in_list_prop)
+
+           apply(subgoal_tac "x64_decode 0 l_bin0 = Some (1,Ppushl_r RCX)")
+                      apply auto[1]
+                     apply(subgoal_tac "list_in_list (x64_encode (Ppushl_r RCX)) 0 l_bin0",simp_all)
+        apply (meson list_in_list_concat list_in_list_prop)
+
+           apply(subgoal_tac "x64_decode 0 l_bin0 = Some (1,Ppushl_r RCX)")
+                      apply auto[1]
+                     apply(subgoal_tac "list_in_list (x64_encode (Ppushl_r RCX)) 0 l_bin0",simp_all)
+        apply (meson list_in_list_concat list_in_list_prop)
+
+           apply(subgoal_tac "x64_decode 0 l_bin0 = Some (1,Ppushl_r RCX)")
+                      apply auto[1]
+                     apply(subgoal_tac "list_in_list (x64_encode (Ppushl_r RCX)) 0 l_bin0",simp_all)
+        apply (meson list_in_list_concat list_in_list_prop)
+
+           apply(subgoal_tac "x64_decode 0 l_bin0 = Some (1,Ppushl_r RCX)")
+                      apply auto[1]
+                     apply(subgoal_tac "list_in_list (x64_encode (Ppushl_r RCX)) 0 l_bin0",simp_all)
+        apply (meson list_in_list_concat list_in_list_prop)
+      done
+ apply(cases x93,simp_all)
+    subgoal for x2
+      apply(cases "bpf_to_x64_reg x92",simp_all)
+apply(subgoal_tac "x64_decode 0 l_bin0 = Some (1,Ppushl_r RCX)")
+                      apply auto[1]
+                     apply(subgoal_tac "list_in_list (x64_encode (Ppushl_r RCX)) 0 l_bin0",simp_all)
+                     apply (meson list_in_list_concat list_in_list_prop)
+apply(subgoal_tac "x64_decode 0 l_bin0 = Some (1,Ppushl_r RCX)")
+                      apply auto[1]
+                     apply(subgoal_tac "list_in_list (x64_encode (Ppushl_r RCX)) 0 l_bin0",simp_all)
+      apply (meson list_in_list_concat list_in_list_prop)
+                   apply(cases "bpf_to_x64_reg x2",simp_all)
+  apply(subgoal_tac "x64_decode 0 l_bin0 = Some (1,Ppushl_r RAX)")
+                      apply auto[1]
+                     apply(subgoal_tac "list_in_list (x64_encode (Ppushl_r RAX)) 0 l_bin0",simp_all)
+                          apply (meson list_in_list_concat list_in_list_prop)
+            apply(subgoal_tac "x64_decode 0 l_bin0 = Some (1,Ppushl_r RBX)")
+                      apply auto[1]
+                     apply(subgoal_tac "list_in_list (x64_encode (Ppushl_r RBX)) 0 l_bin0",simp_all)
+                     apply (meson list_in_list_concat list_in_list_prop)
+            apply(subgoal_tac "x64_decode 0 l_bin0 = Some (1,Ppushl_r RDX)")
+                      apply auto[1]
+                     apply(subgoal_tac "list_in_list (x64_encode (Ppushl_r RDX)) 0 l_bin0",simp_all)
+                          apply (meson list_in_list_concat list_in_list_prop)
+            apply(subgoal_tac "x64_decode 0 l_bin0 = Some (1,Ppushl_r RSI)")
+                      apply auto[1]
+                     apply(subgoal_tac "list_in_list (x64_encode (Ppushl_r RSI)) 0 l_bin0",simp_all)
+                     apply (meson list_in_list_concat list_in_list_prop)
+
+            apply(subgoal_tac "x64_decode 0 l_bin0 = Some (1,Ppushl_r RDI)")
+                      apply auto[1]
+                     apply(subgoal_tac "list_in_list (x64_encode (Ppushl_r RDI)) 0 l_bin0",simp_all)
+                          apply (meson list_in_list_concat list_in_list_prop)
+                          apply(subgoal_tac "x64_decode 0 l_bin0 = Some (1,Ppushl_r RBP)")
+                      apply auto[1]
+                     apply(subgoal_tac "list_in_list (x64_encode (Ppushl_r RBP)) 0 l_bin0",simp_all)
+                          apply (meson list_in_list_concat list_in_list_prop)
+              apply(subgoal_tac "x64_decode 0 l_bin0 = Some (1,Ppushl_r SP)")
+                      apply auto[1]
+                     apply(subgoal_tac "list_in_list (x64_encode (Ppushl_r SP)) 0 l_bin0",simp_all)
+                          apply (meson list_in_list_concat list_in_list_prop)
+              apply(subgoal_tac "x64_decode 0 l_bin0 = Some (1,Ppushl_r R8)")
+                      apply auto[1]
+                     apply(subgoal_tac "list_in_list (x64_encode (Ppushl_r R8)) 0 l_bin0",simp_all)
+                          apply (meson list_in_list_concat list_in_list_prop)
+              apply(subgoal_tac "x64_decode 0 l_bin0 = Some (1,Ppushl_r R9)")
+                      apply auto[1]
+                     apply(subgoal_tac "list_in_list (x64_encode (Ppushl_r R9)) 0 l_bin0",simp_all)
+                         apply (meson list_in_list_concat list_in_list_prop)
+              apply(subgoal_tac "x64_decode 0 l_bin0 = Some (1,Ppushl_r REG_OTHER_SCRATCH)")
+                      apply auto[1]
+                     apply(subgoal_tac "list_in_list (x64_encode (Ppushl_r REG_OTHER_SCRATCH)) 0 l_bin0",simp_all)
+                        apply (meson list_in_list_concat list_in_list_prop)
+        apply(subgoal_tac "x64_decode 0 l_bin0 = Some (1,Ppushl_r REG_SCRATCH)")
+                      apply auto[1]
+                     apply(subgoal_tac "list_in_list (x64_encode (Ppushl_r REG_SCRATCH)) 0 l_bin0",simp_all)
+                       apply (meson list_in_list_concat list_in_list_prop)
+        apply(subgoal_tac "x64_decode 0 l_bin0 = Some (1,Ppushl_r R12)")
+                      apply auto[1]
+                     apply(subgoal_tac "list_in_list (x64_encode (Ppushl_r R12)) 0 l_bin0",simp_all)
+                      apply (meson list_in_list_concat list_in_list_prop)
+
+   apply(subgoal_tac "x64_decode 0 l_bin0 = Some (1,Ppushl_r R13)")
+                      apply auto[1]
+                     apply(subgoal_tac "list_in_list (x64_encode (Ppushl_r R13)) 0 l_bin0",simp_all)
+        apply (meson list_in_list_concat list_in_list_prop)
+           apply(subgoal_tac "x64_decode 0 l_bin0 = Some (1,Ppushl_r R14)")
+                      apply auto[1]
+                     apply(subgoal_tac "list_in_list (x64_encode (Ppushl_r R14)) 0 l_bin0",simp_all)
+                    apply (meson list_in_list_concat list_in_list_prop)
+           apply(subgoal_tac "x64_decode 0 l_bin0 = Some (1,Ppushl_r R15)")
+                      apply auto[1]
+                     apply(subgoal_tac "list_in_list (x64_encode (Ppushl_r R15)) 0 l_bin0",simp_all)
+                   apply (meson list_in_list_concat list_in_list_prop)
+           apply(subgoal_tac "x64_decode 0 l_bin0 = Some (1,Ppushl_r RCX)")
+                      apply auto[1]
+                     apply(subgoal_tac "list_in_list (x64_encode (Ppushl_r RCX)) 0 l_bin0",simp_all)
+                  apply (meson list_in_list_concat list_in_list_prop)
+           apply(subgoal_tac "x64_decode 0 l_bin0 = Some (1,Ppushl_r RCX)")
+                      apply auto[1]
+                     apply(subgoal_tac "list_in_list (x64_encode (Ppushl_r RCX)) 0 l_bin0",simp_all)
+        apply (meson list_in_list_concat list_in_list_prop)
+           apply(subgoal_tac "x64_decode 0 l_bin0 = Some (1,Ppushl_r RCX)")
+                      apply auto[1]
+                     apply(subgoal_tac "list_in_list (x64_encode (Ppushl_r RCX)) 0 l_bin0",simp_all)
+        apply (meson list_in_list_concat list_in_list_prop)
+
+           apply(subgoal_tac "x64_decode 0 l_bin0 = Some (1,Ppushl_r RCX)")
+                      apply auto[1]
+                     apply(subgoal_tac "list_in_list (x64_encode (Ppushl_r RCX)) 0 l_bin0",simp_all)
+        apply (meson list_in_list_concat list_in_list_prop)
+
+           apply(subgoal_tac "x64_decode 0 l_bin0 = Some (1,Ppushl_r RCX)")
+                      apply auto[1]
+                     apply(subgoal_tac "list_in_list (x64_encode (Ppushl_r RCX)) 0 l_bin0",simp_all)
+        apply (meson list_in_list_concat list_in_list_prop)
+
+           apply(subgoal_tac "x64_decode 0 l_bin0 = Some (1,Ppushl_r RCX)")
+                      apply auto[1]
+                     apply(subgoal_tac "list_in_list (x64_encode (Ppushl_r RCX)) 0 l_bin0",simp_all)
+        apply (meson list_in_list_concat list_in_list_prop)
+
+           apply(subgoal_tac "x64_decode 0 l_bin0 = Some (1,Ppushl_r RCX)")
+                      apply auto[1]
+                     apply(subgoal_tac "list_in_list (x64_encode (Ppushl_r RCX)) 0 l_bin0",simp_all)
+        apply (meson list_in_list_concat list_in_list_prop)
+
+           apply(subgoal_tac "x64_decode 0 l_bin0 = Some (1,Ppushl_r RCX)")
+                      apply auto[1]
+                     apply(subgoal_tac "list_in_list (x64_encode (Ppushl_r RCX)) 0 l_bin0",simp_all)
+        apply (meson list_in_list_concat list_in_list_prop)
+
+           apply(subgoal_tac "x64_decode 0 l_bin0 = Some (1,Ppushl_r RCX)")
+                      apply auto[1]
+                     apply(subgoal_tac "list_in_list (x64_encode (Ppushl_r RCX)) 0 l_bin0",simp_all)
+        apply (meson list_in_list_concat list_in_list_prop)
+
+           apply(subgoal_tac "x64_decode 0 l_bin0 = Some (1,Ppushl_r RCX)")
+                      apply auto[1]
+                     apply(subgoal_tac "list_in_list (x64_encode (Ppushl_r RCX)) 0 l_bin0",simp_all)
+        apply (meson list_in_list_concat list_in_list_prop)
+
+           apply(subgoal_tac "x64_decode 0 l_bin0 = Some (1,Ppushl_r RCX)")
+                      apply auto[1]
+                     apply(subgoal_tac "list_in_list (x64_encode (Ppushl_r RCX)) 0 l_bin0",simp_all)
+        apply (meson list_in_list_concat list_in_list_prop)
+
+           apply(subgoal_tac "x64_decode 0 l_bin0 = Some (1,Ppushl_r RCX)")
+                      apply auto[1]
+                     apply(subgoal_tac "list_in_list (x64_encode (Ppushl_r RCX)) 0 l_bin0",simp_all)
+        apply (meson list_in_list_concat list_in_list_prop)
+
+           apply(subgoal_tac "x64_decode 0 l_bin0 = Some (1,Ppushl_r RCX)")
+                      apply auto[1]
+                     apply(subgoal_tac "list_in_list (x64_encode (Ppushl_r RCX)) 0 l_bin0",simp_all)
+        apply (meson list_in_list_concat list_in_list_prop)
+      done
+    apply(cases x93,simp_all)
+    subgoal for x2
+      apply(cases "bpf_to_x64_reg x92",simp_all)
+      apply(subgoal_tac "x64_decode 0 l_bin0 = Some (3,Pmovq_rr REG_SCRATCH (bpf_to_x64_reg x2))")
+       apply auto[1]
+      apply(subgoal_tac "list_in_list (x64_encode (Pmovq_rr REG_SCRATCH (bpf_to_x64_reg x2))) 0 l_bin0",simp_all)                   
+                     apply (meson list_in_list_concat list_in_list_prop)
+ apply(subgoal_tac "x64_decode 0 l_bin0 = Some (3,Pmovq_rr REG_SCRATCH (bpf_to_x64_reg x2))")
+       apply auto[1]
+      apply(subgoal_tac "list_in_list (x64_encode (Pmovq_rr REG_SCRATCH (bpf_to_x64_reg x2))) 0 l_bin0",simp_all)                   
+                    apply (meson list_in_list_concat list_in_list_prop)
+ apply(subgoal_tac "x64_decode 0 l_bin0 = Some (3,Pmovq_rr REG_SCRATCH (bpf_to_x64_reg x2))")
+       apply auto[1]
+      apply(subgoal_tac "list_in_list (x64_encode (Pmovq_rr REG_SCRATCH (bpf_to_x64_reg x2))) 0 l_bin0",simp_all)                   
+                   apply (meson list_in_list_concat list_in_list_prop)
+ apply(subgoal_tac "x64_decode 0 l_bin0 = Some (3,Pmovq_rr REG_SCRATCH (bpf_to_x64_reg x2))")
+       apply auto[1]
+      apply(subgoal_tac "list_in_list (x64_encode (Pmovq_rr REG_SCRATCH (bpf_to_x64_reg x2))) 0 l_bin0",simp_all)                   
+                  apply (meson list_in_list_concat list_in_list_prop)
+ apply(subgoal_tac "x64_decode 0 l_bin0 = Some (3,Pmovq_rr REG_SCRATCH (bpf_to_x64_reg x2))")
+       apply auto[1]
+      apply(subgoal_tac "list_in_list (x64_encode (Pmovq_rr REG_SCRATCH (bpf_to_x64_reg x2))) 0 l_bin0",simp_all)                   
+                 apply (meson list_in_list_concat list_in_list_prop)
+ apply(subgoal_tac "x64_decode 0 l_bin0 = Some (3,Pmovq_rr REG_SCRATCH (bpf_to_x64_reg x2))")
+       apply auto[1]
+      apply(subgoal_tac "list_in_list (x64_encode (Pmovq_rr REG_SCRATCH (bpf_to_x64_reg x2))) 0 l_bin0",simp_all)                   
+                apply (meson list_in_list_concat list_in_list_prop)
+ apply(subgoal_tac "x64_decode 0 l_bin0 = Some (3,Pmovq_rr REG_SCRATCH (bpf_to_x64_reg x2))")
+       apply auto[1]
+      apply(subgoal_tac "list_in_list (x64_encode (Pmovq_rr REG_SCRATCH (bpf_to_x64_reg x2))) 0 l_bin0",simp_all)                   
+               apply (meson list_in_list_concat list_in_list_prop)
+ apply(subgoal_tac "x64_decode 0 l_bin0 = Some (3,Pmovq_rr REG_SCRATCH (bpf_to_x64_reg x2))")
+       apply auto[1]
+      apply(subgoal_tac "list_in_list (x64_encode (Pmovq_rr REG_SCRATCH (bpf_to_x64_reg x2))) 0 l_bin0",simp_all)                   
+              apply (meson list_in_list_concat list_in_list_prop)
+ apply(subgoal_tac "x64_decode 0 l_bin0 = Some (3,Pmovq_rr REG_SCRATCH (bpf_to_x64_reg x2))")
+       apply auto[1]
+      apply(subgoal_tac "list_in_list (x64_encode (Pmovq_rr REG_SCRATCH (bpf_to_x64_reg x2))) 0 l_bin0",simp_all)                   
+             apply (meson list_in_list_concat list_in_list_prop)
+ apply(subgoal_tac "x64_decode 0 l_bin0 = Some (3,Pmovq_rr REG_SCRATCH (bpf_to_x64_reg x2))")
+       apply auto[1]
+      apply(subgoal_tac "list_in_list (x64_encode (Pmovq_rr REG_SCRATCH (bpf_to_x64_reg x2))) 0 l_bin0",simp_all)                   
+            apply (meson list_in_list_concat list_in_list_prop)
+ apply(subgoal_tac "x64_decode 0 l_bin0 = Some (3,Pmovq_rr REG_SCRATCH (bpf_to_x64_reg x2))")
+       apply auto[1]
+      apply(subgoal_tac "list_in_list (x64_encode (Pmovq_rr REG_SCRATCH (bpf_to_x64_reg x2))) 0 l_bin0",simp_all)                   
+           apply (meson list_in_list_concat list_in_list_prop)
+ apply(subgoal_tac "x64_decode 0 l_bin0 = Some (3,Pmovq_rr REG_SCRATCH (bpf_to_x64_reg x2))")
+       apply auto[1]
+      apply(subgoal_tac "list_in_list (x64_encode (Pmovq_rr REG_SCRATCH (bpf_to_x64_reg x2))) 0 l_bin0",simp_all)                   
+          apply (meson list_in_list_concat list_in_list_prop)
+ apply(subgoal_tac "x64_decode 0 l_bin0 = Some (3,Pmovq_rr REG_SCRATCH (bpf_to_x64_reg x2))")
+       apply auto[1]
+      apply(subgoal_tac "list_in_list (x64_encode (Pmovq_rr REG_SCRATCH (bpf_to_x64_reg x2))) 0 l_bin0",simp_all)                   
+         apply (meson list_in_list_concat list_in_list_prop)
+ apply(subgoal_tac "x64_decode 0 l_bin0 = Some (3,Pmovq_rr REG_SCRATCH (bpf_to_x64_reg x2))")
+       apply auto[1]
+      apply(subgoal_tac "list_in_list (x64_encode (Pmovq_rr REG_SCRATCH (bpf_to_x64_reg x2))) 0 l_bin0",simp_all)                   
+        apply (meson list_in_list_concat list_in_list_prop)
+ apply(subgoal_tac "x64_decode 0 l_bin0 = Some (3,Pmovq_rr REG_SCRATCH (bpf_to_x64_reg x2))")
+       apply auto[1]
+      apply(subgoal_tac "list_in_list (x64_encode (Pmovq_rr REG_SCRATCH (bpf_to_x64_reg x2))) 0 l_bin0",simp_all)                   
+       apply (meson list_in_list_concat list_in_list_prop)
+ apply(subgoal_tac "x64_decode 0 l_bin0 = Some (3,Pmovq_rr REG_SCRATCH (bpf_to_x64_reg x2))")
+       apply auto[1]
+      apply(subgoal_tac "list_in_list (x64_encode (Pmovq_rr REG_SCRATCH (bpf_to_x64_reg x2))) 0 l_bin0",simp_all)                   
+                     apply (meson list_in_list_concat list_in_list_prop)
+      done
+    done
+  done
+
+
+
+lemma jit_prog_prop4:
+  "jitper insns = Some lt \<Longrightarrow> 
+  lt!(unat pc) = (num,off,l_bin0) \<Longrightarrow> 
+  unat pc < length lt \<and> unat pc \<ge> 0 \<Longrightarrow> 
+  \<exists> src dst. x64_decode 0 l_bin0 = Some(3, Pcmpq_rr src dst) \<Longrightarrow> 
+  num = 1"
+
+  proof(induct lt arbitrary:insns pc num off l_bin0)
+    case Nil
+    then show ?case by simp
+  next
+    case (Cons a lt)
+    assume assm0: "jitper insns = Some (a#lt)" and
+      assm1:"(a#lt)!(unat pc) = (num,off,l_bin0)" and
+      assm2:"unat pc < length (a#lt) \<and> unat pc \<ge> 0" and
+      assm3:"\<exists> src dst. x64_decode 0 l_bin0 = Some(3, Pcmpq_rr src dst)"
+    have a0:"unat pc = 0 \<or> unat pc \<ge> 1" by auto
+    show ?case
+    proof (cases "unat pc = 0")
+      case True
+      have b0:"\<exists> ins. per_jit_ins ins = Some a" using Cons
+        by (smt (verit) True aux5 is_none_code(2) is_none_simps(1) jitper.elims length_greater_0_conv list.simps(3) nth_Cons_0 option.inject option.split_sel) 
+      then obtain ins where b1:"per_jit_ins ins = Some a" by auto
+      then show ?thesis using jit_prog_prop2
+        using True assm3 local.Cons(3) by auto 
+    next
+      case False
+      let "?pc" = "unat pc -1"
+      have b0:"unat pc \<ge> 1" using False a0 by simp     
+      hence b1:"0 \<le> ?pc \<and> ?pc < length lt \<and> lt!(?pc) = (num,off,l_bin0)"
+        by (metis (no_types, lifting) False One_nat_def assm1 assm2 less_diff_conv2 list.size(4) nth_Cons' zero_le) 
+      have b2_1:"insns \<noteq> []" using assm0 by force
+      let "?ins" = "hd insns"
+      have b2:"per_jit_ins ?ins = Some a" using assm0 b2_1
+        by (metis (no_types, lifting) aux5 is_none_code(2) is_none_simps(1) jitper.elims length_greater_0_conv list.sel(1) nth_Cons_0 option.collapse option.simps(4) unsigned_0 zero_order(1)) 
+      let "?prog" = "tl insns"
+      have b2_2:"?ins#?prog = insns" by (simp add: b2_1) 
+      have "jitper ?prog = Some lt" using assm0 b2_1 b2 apply(cases "per_jit_ins ?ins",simp_all) apply(cases "jitper ?prog",simp_all)
+         apply (metis (no_types, lifting) b2_2 jitper.simps(2) not_None_eq old.prod.case option.simps(4) option.simps(5) split_pairs) 
+        subgoal for aa by (metis (no_types, lifting) b2_2 jitper.simps(2) list.sel(3) old.prod.case option.simps(5) prod.collapse) 
+        done
+        thus ?thesis using b0 b1 by (metis (no_types, lifting) Cons.hyps False local.Cons(5) unat_minus_one unsigned_0 zero_le)       
+      qed     
+    qed
+
+lemma "jitper insns = Some lt \<Longrightarrow> lt \<noteq> [] \<Longrightarrow> well_formed_prog1 lt"
+  using jit_prog_prop3 well_formed_prog1_def sorry
+             
+(*
+lemma jit_prog_prop1:"x64_encode ins \<noteq> undefined \<Longrightarrow>  x64_encode ins \<noteq> []"
+  apply(unfold x64_encode_def)
+  apply(cases ins,simp_all)
+  subgoal for x7 
+    apply(unfold construct_rex_to_u8_def Let_def,simp_all)
+    done
+  subgoal for x8
+    apply(unfold construct_rex_to_u8_def Let_def,simp_all)
+    done
+  subgoal for x111 x112
+apply(unfold construct_rex_to_u8_def Let_def,simp_all)
+    done
+  subgoal for x151 x152 x153
+    apply(cases x151,simp_all)
+    subgoal for x1 x2 x3 
+      apply(cases x1,simp_all) 
+      subgoal for a apply(cases x2,simp_all)
+         apply(unfold construct_rex_to_u8_def Let_def,simp_all)
+        sorry
+      done
+    done
+  subgoal for x201 x202 x203
+    apply(cases x202,simp_all) 
+    subgoal for x1 x2 x3
+      apply(cases x1,simp_all) 
+      subgoal apply(cases x2,simp_all) 
+         apply(unfold construct_rex_to_u8_def Let_def,simp_all)
+         apply(cases x203,simp_all) 
+        sorry
+    done
+  done
+*)
+
+(*lemma "jitper insns = Some lt \<Longrightarrow> insns \<noteq> [] \<Longrightarrow> lt \<noteq> []"
+  using jit_prog_prop3 *)
+
+end
