theory/JITFlattern_prob.thy
@@ -114,6 +114,9 @@ lemma x64_bin_is_sequential_x64_decode_pcall_false: "
     done
   done
 
+lemma "x64_decode x l = Some (sz2, Pcall_i x1) \<Longrightarrow> \<not> (x64_bin_is_sequential n l x)"
+  using x64_bin_is_sequential_x64_decode_pcall_false by blast
+
  (*l!x \<noteq> 0xe8 \<and> l!x \<noteq> 0xc3 \<and> l!(x+1) \<noteq> (0x39::u8) \<Longrightarrow>*)
 lemma list_in_list_prop3: "
   x64_sem num l_bin (Next (xpc+x) xrs xm xss) = fxst \<Longrightarrow>
